src/FrameStack/SubstSemanticsLemmas.v
@@ -502,6 +502,7 @@ Proof.
     do 2 (constructor; auto).
   * do 2 (constructor; auto).
     - apply (H5 0). simpl. lia.
+    - eexists; eassumption.
     - intros. apply (H2 (S i)). simpl. lia.
     - intros. apply (H5 (S i)). simpl. lia.
   * constructor. apply -> subst_preserves_scope_exp.
@@ -557,9 +558,29 @@ Proof.
   * apply step_closedness in H; auto. firstorder.
 Qed.
 
+Theorem transitive_eval : forall {n Fs Fs' e e'},
+  ⟨ Fs, e ⟩ -[n]-> ⟨ Fs', e' ⟩ -> forall {n' Fs'' e''}, ⟨ Fs', e' ⟩ -[n']-> ⟨ Fs'', e'' ⟩
+->
+  ⟨ Fs, e ⟩ -[n + n']-> ⟨ Fs'', e''⟩.
+Proof.
+  intros n Fs F' e e' IH. induction IH; intros; auto.
+  simpl. econstructor. exact H. now apply IHIH.
+Qed.
 
 
-
+Lemma terminates_in_k_step :
+  forall fs e fs' e' k, ⟨ fs, e ⟩ --> ⟨ fs', e' ⟩ ->
+  | fs', e' | k ↓ ->
+  | fs, e | S k ↓.
+Proof.
+  intros fs e fs' e' k H H0. induction H.
+  all: try (now constructor).
+  * eapply cool_params_0; eassumption.
+  * eapply cool_params; eassumption.
+  * eapply step_case_match; eassumption.
+  * eapply step_case_true; eassumption.
+  * eapply heat_letrec; eassumption.
+Qed.
 
 Theorem terminates_in_k_eq_terminates_in_k_sem :
   forall k e fs, terminates_in_k_sem fs e k <-> | fs, e | k ↓.
@@ -575,1419 +596,464 @@ Proof.
         eexists. split; eassumption.
       }
       apply IHk in H.
+      eapply terminates_in_k_step; eassumption.
+  }
+  {
+    intros. induction H.
+    all: try destruct IHterminates_in_k as [res0 [Hres0 HD]].
+    all: try (now eexists; split;
+                  [eassumption | econstructor;
+                      [constructor | assumption]]).
+    * eexists. split.
+      - eassumption.
+      - constructor.
+    * eexists. split.
+      - eassumption.
+      - econstructor. constructor; eassumption.
+        eassumption.
+    * eexists. split.
+      - exact Hres0.
+      - econstructor. constructor; eassumption.
+        eassumption.
+    * eexists. split.
+      - eassumption.
+      - econstructor. constructor; eassumption.
+        eassumption.
+    * eexists. split.
+      - eassumption.
+      - econstructor. constructor; eassumption.
+        eassumption.
+    * eexists. split.
+      - eassumption.
+      - econstructor. constructor; eassumption.
+        eassumption.
   }
 Qed.
 
-
-
-
-
-
-
-
-
-
-(** This theorem says that the semantics rules are deterministic. *)
-Theorem semmantics_rules_determinism :
-  forall fs fs1 fs2 e e1 e2,
-  ⟨ fs , e ⟩ --> ⟨ fs1 , e1 ⟩ ->
-  ⟨ fs , e ⟩ --> ⟨ fs2 , e2 ⟩
-  -> (fs1 = fs2 /\ e1 = e2).
+Theorem terminates_step :
+  forall n fs e, | fs, e | n ↓ -> forall fs' e', ⟨fs, e⟩ --> ⟨fs', e'⟩
+->
+  | fs', e' | n - 1↓.
 Proof.
-intros. inversion H; subst; inversion H0; auto; subst.
-* rewrite H1 in H4. inversion H4. subst. auto.
-* rewrite H1 in H4. inversion H4.
-* rewrite H1 in H8. inversion H8. subst. auto.
-* rewrite H1 in H8. inversion H8.
-* rewrite H1 in H4. inversion H4.
-* rewrite H1 in H4. inversion H4. subst. auto.
-* rewrite H1 in H8. inversion H8.
-* rewrite H1 in H8. inversion H8. subst. auto.
-* rewrite H1 in H4. inversion H4. subst. auto.
-* rewrite H1 in H4. inversion H4.
-* rewrite H1 in H8. inversion H8. subst. auto.
-* rewrite H1 in H8. inversion H8.
-* rewrite H1 in H4. inversion H4.
-* rewrite H1 in H4. inversion H4. subst. auto.
-* rewrite H1 in H8. inversion H8.
-* rewrite H1 in H8. inversion H8. subst. auto.
-* auto.
-* congruence.
-* specialize (H3 ext id 0 e0). congruence.
-* auto.
-* congruence.
-* specialize (H7 ext id (Datatypes.length vl + 1) e'). congruence.
-* congruence.
-* specialize (H4 ext id vc e0). congruence.
-* congruence.
-* specialize (H8 ext id vc e'). congruence.
-* specialize (H1 ext id 0 e). congruence.
-* specialize (H1 ext id vc e). congruence.
-* specialize (H1 ext id (Datatypes.length vl + 1) e'). congruence.
-* specialize (H1 ext id vc e'). congruence.
-* rewrite H1 in H10. inversion H10. subst. auto.
-* rewrite H1 in H10. inversion H10.
-* rewrite H1 in H10. inversion H10.
-* auto.
-* specialize (H6 vl1 e0 3 e3). congruence.
-* specialize (H1 vl1 e0 3 e3). congruence.
+  intros. apply terminates_in_k_eq_terminates_in_k_sem in H. destruct H. destruct n.
+  * destruct H. inv H.
+    - subst. inversion H1; subst. inversion H0.
+    - subst. inversion H1; subst. inversion H0.
+  * destruct H.
+    inv H1. subst. apply (step_determinism H0) in H3. inv H3.
+    assert (exists y, is_result y /\ ⟨ fs', e' ⟩ -[ n ]-> ⟨ [], y ⟩). { 
+      eexists. eauto. }
+    apply ex_intro in H6. apply terminates_in_k_eq_terminates_in_k_sem in H1.
+    now rewrite Nat.sub_1_r.
 Qed.
 
-
-Theorem step_rt_determinism :
-  forall e k fs fs1 fs2 r1 r2,
-  ⟨fs, e⟩ -[k]-> ⟨fs1, r1⟩ ->
-  ⟨fs, e⟩ -[k]-> ⟨fs2, r2⟩
-  -> (fs1 = fs2 /\ r1 = r2).
+Corollary term_step_term :
+  forall k n fs e, | fs, e | n ↓ -> forall fs' e', ⟨fs, e⟩ -[k]-> ⟨fs', e'⟩
+->
+  | fs', e' | n - k ↓.
 Proof.
-  intros. dependent induction H.
-  * inversion H0. subst. auto.
-  * inversion H1. subst.
-    pose proof semmantics_rules_determinism.
-    specialize (H2 fs fs' fs'0 e e' e'0 H H3). destruct H2. subst.
-    apply IHstep_rt. auto.
+  induction k; intros; inversion H0; subst; auto.
+  * rewrite Nat.sub_0_r. auto.
+  * apply terminates_step with (n := n) in H2; auto.
+    eapply IHk in H5; auto. 2: exact H2. now replace (n - S k) with ((n - 1) - k) by lia.
 Qed.
 
-
-(*This lemma was stated incorrectl, but the proof only needs some fixing*)
-(*
-Lemma eval_is_closed : 
-  forall f params eff res eff',
-  Auxiliaries.eval f params eff = (inl res, eff') ->
-  (forall i, i < length params -> VALCLOSED (nth i params VNil))
-  -> 
-  (forall i, i < length res -> VALCLOSED (nth i res VNil)).
-Proof.
-  intros. unfold Auxiliaries.eval in H.
-  destruct (convert_string_to_code f) eqn:Hfname; simpl in H.
-  all: try (unfold eval_arith, eval_logical, eval_equality,
-             eval_transform_list, eval_list_tuple, eval_cmp,
-             eval_hd_tl, eval_elem_tuple, eval_check, eval_error, eval_io in H; rewrite Hfname in H);
-  destruct params;
-(* B route *)
-[
-  inversion H |
-  destruct v; try (destruct params; [inversion H | destruct params; inversion H])
-]; try (destruct l; inversion H).
-(*
-try (destruct v; try (subst; inversion H3; subst; inversion H1; [subst; simpl; constructor | lia ]);
-    try (
-    subst; destruct (Equalities.Value_eqb _ _); [inversion H; subst; inversion H1; [ simpl;
-    constructor | lia] | inversion H; subst; inversion H1; [ simpl; constructor | lia] ])).
-*)
-(* try (destruct v; try (subst; inversion H3; subst; inversion H1; [subst; simpl; constructor | lia ])). *)
-  * subst. specialize (H0 i H1). auto.
-  * destruct v; try (inversion H).
-    - destruct l.
-      + inversion H.
-      + inversion H7. subst. destruct i.
-        ** simpl. constructor.
-        ** simpl in H1. lia.
-  * destruct v; try (destruct params; inversion H).
-    - destruct l; inversion H.
-    - destruct l; inversion H.
-  * subst. specialize (H0 i H1). destruct i.
-    - simpl. constructor.
-    - simpl in H1. lia.
-  * destruct v; inversion H.
-    - destruct l.
-      + inversion H.
-      + inversion H. subst. simpl in *. specialize (H0 i H1). inversion H1.
-        ** subst. simpl. constructor.
-        ** lia.
-  * destruct v; inversion H.
-    - destruct l; inversion H.
-  * destruct v; inversion H.
-    - destruct l; inversion H.
-      + subst. specialize (H0 i H1). inversion H1.
-        ** subst. simpl. constructor.
-        ** lia.
-  * destruct v; inversion H.
-    - destruct l; inversion H.
-  * destruct v; inversion H.
-    - destruct l; inversion H.
-      + destruct x0; inversion H.
-        ** subst. specialize (H0 i H1). inversion H1.
-           -- subst. simpl. constructor.
-           -- lia.
-        ** subst. specialize (H0 i H1). inversion H1.
-           -- subst. simpl. constructor.
-           -- lia.
-  * destruct v; inversion H.
-    - destruct l; inversion H.
-      + destruct x0; inversion H.
-  * destruct v; inversion H.
-    - destruct l; inversion H.
-      + destruct x0; inversion H.
-        ** subst. specialize (H0 i H1). inversion H1.
-           -- subst. simpl. constructor.
-           -- lia.
-        ** subst. specialize (H0 i H1). inversion H1.
-           -- subst. simpl. constructor.
-           -- lia.
-  * destruct v; inversion H.
-    - destruct l; inversion H.
-      + destruct x0; inversion H.
-  * destruct v; inversion H.
-    - destruct l; inversion H.
-      + destruct x0; inversion H.
-        ** subst. specialize (H0 i H1). inversion H1.
-           -- subst. simpl. constructor.
-           -- lia.
-        ** subst. specialize (H0 i H1). inversion H1.
-           -- subst. simpl. constructor.
-           -- lia.
-  * destruct v; inversion H.
-    - destruct l; inversion H.
-      + destruct x0; inversion H.
-  * destruct v; inversion H.
-    - destruct l; inversion H.
-      + subst. specialize (H0 i H1). inversion H1.
-        ** subst. simpl. constructor.
-        ** lia.
-  * destruct v; inversion H.
-    - destruct l; inversion H.
-  * destruct v; inversion H.
-    - destruct l; inversion H.
-      + subst. specialize (H0 i H1). inversion H1.
-        ** subst. simpl. constructor.
-        ** lia.
-  * destruct v; inversion H.
-    - destruct l; inversion H.
-  
-  * subst. specialize (H0 i H1).  inversion H1.
-    - subst. simpl. constructor.
-    - lia.
-  * simpl in H; subst; unfold ok; inversion H1; [subst; simpl; constructor | lia ].
-  * simpl in H; subst; unfold ok; inversion H1; [subst; simpl; constructor | lia ].
-  * simpl in H; subst; unfold ok; inversion H1; [subst; simpl; constructor | lia ].
-  * simpl in H; subst; unfold ok; inversion H1; [subst; simpl; constructor | lia ].
-  * simpl in H; subst; unfold ok; inversion H1; [subst; simpl; constructor | lia ].
-  * simpl in H; subst; unfold ok; inversion H1; [subst; simpl; constructor | lia ].
-  * simpl in H; subst; unfold ok; inversion H1; [subst; simpl; constructor | lia ].
-  * simpl in H; subst; unfold ok; inversion H1; [subst; simpl; constructor | lia ].
-  * simpl in H; subst; unfold ok; inversion H1; [subst; simpl; constructor | lia ].
-  * simpl in H; subst; unfold ok; inversion H1; [subst; simpl; constructor | lia ].
-  * simpl in H; subst; unfold ok; inversion H1; [subst; simpl; constructor | lia ].
-  * simpl in H. subst. unfold ok. inversion H1.
-    - subst. simpl. constructor. intros. destruct i.
-      + simpl. constructor.
-      + destruct i.
-        ** simpl. admit. (* use H0 *) (* The problem is "i < Datatypes.length [VTuple [ok; v]]" -> i=0 and I need i=1 for VALCLOSED v*)
-        ** simpl in H2. lia.
-    - lia.
-  * simpl in H. subst. unfold ok. inversion H1.
-    - subst. simpl. constructor. intros. destruct i.
-      + simpl. constructor.
-      + destruct i.
-        ** simpl. admit. (* I need i=1 in H0 but i=0*)
-        ** simpl in H2. lia.
-    - lia.
-  * simpl in H. subst. unfold ok. inversion H1.
-    - subst. simpl. constructor. admit.
-    - lia.
-  * simpl in H. subst. unfold ok. inversion H1.
-    - subst. simpl. constructor. admit.
-    - lia.
-  * simpl in H. subst. unfold ok. inversion H1.
-    - subst. simpl. constructor. admit.
-    - lia.
-  * simpl in H. subst. unfold ok. inversion H1.
-    - subst. simpl. constructor. admit.
-    - lia.
-  * simpl in H. subst. unfold ok. inversion H1.
-    - subst. simpl. constructor. admit.
-    - lia.
-  * simpl in H. subst. unfold ok. inversion H1.
-    - subst. simpl. constructor. admit.
-    - lia.
-  * simpl in H. subst. unfold ok. inversion H1.
-    - subst. simpl. constructor. admit.
-    - lia.
-  * simpl in H. subst. unfold ok. inversion H1.
-    - subst. simpl. constructor. admit.
-    - lia.
-  * simpl in H. subst. unfold ok. inversion H1.
-    - subst. simpl. constructor. admit.
-    - lia.
-  (* New bool evaluation method *)
-  * unfold ttrue in *. unfold ffalse in *.
-    destruct (Equalities.Value_eqb (VLit (Atom s)) (VLit (Atom "true"))).
-    - destruct (Equalities.Value_eqb v (VLit (Atom "true"))).
-      + inversion H. subst. inversion H1.
-        ** subst. simpl. constructor.
-        ** lia.
-      + destruct (Equalities.Value_eqb v (VLit (Atom "false"))).
-        ** inversion H. subst. inversion H1.
-           -- subst. simpl. constructor.
-           -- lia.
-        ** inversion H.
-    - destruct (Equalities.Value_eqb (VLit (Atom s)) (VLit (Atom "false"))).
-      + destruct (Equalities.Value_eqb v (VLit (Atom "true"))).
-        ** inversion H. subst. inversion H1.
-           -- subst. simpl. constructor.
-           -- lia.
-        ** destruct (Equalities.Value_eqb v (VLit (Atom "false"))).
-           -- inversion H. subst. inversion H1.
-              ++ subst. simpl. constructor.
-              ++ lia.
-           -- inversion H.
-       + inversion H.
-  * unfold ttrue in *. unfold ffalse in *.
-    destruct (Equalities.Value_eqb (VLit (Atom s)) (VLit (Atom "true"))).
-    - destruct (Equalities.Value_eqb v (VLit (Atom "true"))).
-      + inversion H. subst. inversion H1.
-        ** subst. simpl. constructor.
-        ** lia.
-      + destruct (Equalities.Value_eqb v (VLit (Atom "false"))).
-        ** inversion H. subst. inversion H1.
-           -- subst. simpl. constructor.
-           -- lia.
-        ** inversion H.
-    - destruct (Equalities.Value_eqb (VLit (Atom s)) (VLit (Atom "false"))).
-      + destruct (Equalities.Value_eqb v (VLit (Atom "true"))).
-        ** inversion H. subst. inversion H1.
-           -- subst. simpl. constructor.
-           -- lia.
-        ** destruct (Equalities.Value_eqb v (VLit (Atom "false"))).
-           -- inversion H. subst. inversion H1.
-              ++ subst. simpl. constructor.
-              ++ lia.
-           -- inversion H.
-       + inversion H.
-  * unfold ttrue in *. unfold ffalse in *.
-    destruct (Equalities.Value_eqb (VLit (Atom s)) (VLit (Atom "true"))).
-    - inversion H. subst. inversion H1.
-      + subst. simpl. constructor.
-      + lia.
-    - destruct (Equalities.Value_eqb (VLit (Atom s)) (VLit (Atom "false"))).
-      + inversion H. subst. inversion H1.
-        ** subst. simpl. constructor.
-        ** lia.
-      + inversion H.
-  
-  (* --------------------------Proof structure starts here----------------------------------- *)
-  * destruct v; try (subst; inversion H3; subst; inversion H1; [subst; simpl; constructor | lia]).
-  * destruct v; try (subst; inversion H3; subst; inversion H1; [subst; simpl; constructor | lia]).
-    - destruct l.
-      + destruct (Equalities.Value_eqb (VLit (Atom s))
-        (VLit (Atom s0))).
-        ** subst. inversion H. subst. inversion H1.
-           -- subst. simpl. constructor.
-           -- lia.
-        ** subst. inversion H. subst. inversion H1.
-           -- subst. simpl. constructor.
-           -- lia.
-      + inversion H5. subst. inversion H1.
-        ** subst. simpl. constructor.
-        ** lia.
-  * destruct v; try (subst; inversion H3; subst; inversion H1; [subst; simpl; constructor | lia]).
-    - destruct l.
-      + subst. inversion H5. subst. inversion H1.
-        ** subst. simpl. constructor.
-        ** lia.
-      + destruct (x =? x0)%Z.
-        ** subst. inversion H5. subst. inversion H1.
-           -- subst. simpl. constructor.
-           -- lia.
-        ** subst. inversion H5. subst. inversion H1.
-           -- subst. simpl. constructor.
-           -- lia.
-  * destruct v; try (subst; inversion H3; subst; inversion H1; [subst; simpl; constructor | lia]).
-    - subst. destruct (Equalities.Value_eqb v1 v3 &&
-        Equalities.Value_eqb v2 v4)%bool.
-      + inversion H3. subst. inversion H1.
-        ** subst. simpl. constructor.
-        ** lia.
-      + inversion H3. subst. inversion H1.
-        ** subst. simpl. constructor.
-        ** lia.
-  * destruct v; try (subst; inversion H3; subst; inversion H1; [subst; simpl; constructor | lia]).
-    - subst. destruct l.
-      + subst. simpl. inversion H5. subst. inversion H1.
-        ** subst. simpl. constructor.
-        ** lia.
-      + subst. simpl. inversion H5. subst. inversion H1.
-        ** subst. simpl. constructor.
-        ** lia.
-  * destruct v; try (subst; inversion H3; subst; inversion H1; [subst; simpl; constructor | lia]).
-    - destruct l0.
-      + subst. inversion H5. subst. inversion H1.
-        ** subst. simpl. constructor.
-        ** lia.
-      + destruct l.
-        ** destruct l0.
-           -- destruct (Equalities.Value_eqb v0 v && true)%bool.
-              ++ subst. inversion H5. subst. inversion H1.
-                 *** subst. simpl. constructor.
-                 *** lia.
-              ++ subst. inversion H5. subst. inversion H1.
-                 *** subst. simpl. constructor.
-                 *** lia.
-           -- destruct (Equalities.Value_eqb v0 v && false)%bool.
-              ++ subst. inversion H5. subst. inversion H1.
-                 *** subst. simpl. constructor.
-                 *** lia.
-              ++ subst. inversion H5. subst. inversion H1.
-                 *** subst. simpl. constructor.
-                 *** lia.
-        ** destruct l0.
-           -- destruct (Equalities.Value_eqb v0 v && false)%bool.
-              ++ subst. inversion H5. subst. inversion H1.
-                 *** subst. simpl. constructor.
-                 *** lia.
-              ++ subst. inversion H5. subst. inversion H1.
-                 *** subst. simpl. constructor.
-                 *** lia.
-           -- destruct l.
-              ++ destruct l0.
-                 *** destruct (Equalities.Value_eqb v0 v &&
-                     (Equalities.Value_eqb v1 v2 && true))%bool.
-                     --- subst. inversion H5. subst. inversion H1.
-                         +++ subst. simpl. constructor.
-                         +++ lia.
-                     --- subst. inversion H5. subst. inversion H1.
-                         +++ subst. simpl. constructor.
-                         +++ lia.
-                 *** destruct (Equalities.Value_eqb v0 v &&
-                     (Equalities.Value_eqb v1 v2 && false))%bool.
-                     --- subst. inversion H5. subst. inversion H1.
-                         +++ subst. simpl. constructor.
-                         +++ lia.
-                     --- subst. inversion H5. subst. inversion H1.
-                         +++ subst. simpl. constructor.
-                         +++ lia.
-              ++ admit.
-  * destruct v; try (subst; inversion H3; subst; inversion H1; [subst; simpl; constructor | lia ]);
-    subst; destruct (Equalities.Value_eqb _ _); [inversion H; subst; inversion H1; [ simpl;
-    constructor | lia] | inversion H; subst; inversion H1; [ simpl; constructor | lia] ].
-  * destruct v; try (subst; inversion H3; subst; inversion H1; [subst; simpl; constructor | lia ]);
-    subst; destruct (Equalities.Value_eqb _ _); [inversion H; subst; inversion H1; [ simpl;
-    constructor | lia] | inversion H; subst; inversion H1; [ simpl; constructor | lia] ].
-  * destruct v; try (subst; inversion H3; subst; inversion H1; [subst; simpl; constructor | lia ]);
-    subst; destruct (Equalities.Value_eqb _ _); [inversion H; subst; inversion H1; [ simpl;
-    constructor | lia] | inversion H; subst; inversion H1; [ simpl; constructor | lia] ].
-  (* * destruct v; inversion H3; subst; inversion H1; subst; try (lia); try (constructor). *)
-  * destruct v; try (subst; inversion H3; subst; inversion H1; [subst; simpl; constructor | lia ]);
-    subst; destruct (Equalities.Value_eqb _ _); [inversion H; subst; inversion H1; [ simpl;
-    constructor | lia] | inversion H; subst; inversion H1; [ simpl; constructor | lia] ].
-  * destruct v; try (subst; inversion H3; subst; inversion H1; [subst; simpl; constructor | lia ]);
-    subst; destruct (Equalities.Value_eqb _ _); [inversion H; subst; inversion H1; [ simpl;
-    constructor | lia] | inversion H; subst; inversion H1; [ simpl; constructor | lia] ].
-  * destruct v; try (subst; inversion H3; subst; inversion H1; [subst; simpl; constructor | lia ]).
-  * destruct v; try (subst; inversion H3; subst; inversion H1; [subst; simpl; constructor | lia ]);
-    subst; destruct (Equalities.Value_eqb _ _); [inversion H; subst; inversion H1; [ simpl;
-    constructor | lia] | inversion H; subst; inversion H1; [ simpl; constructor | lia] ].
-  * destruct v; try (subst; inversion H3; subst; inversion H1; [subst; simpl; constructor | lia ]);
-    subst; destruct (Equalities.Value_eqb _ _); [inversion H; subst; inversion H1; [ simpl;
-    constructor | lia] | inversion H; subst; inversion H1; [ simpl; constructor | lia] ].
-  * destruct v; try (subst; inversion H3; subst; inversion H1; [subst; simpl; constructor | lia ]);
-    subst; destruct (Equalities.Value_eqb _ _); [inversion H; subst; inversion H1; [ simpl;
-    constructor | lia] | inversion H; subst; inversion H1; [ simpl; constructor | lia] ].
-  * destruct v; try (subst; inversion H3; subst; inversion H1; [subst; simpl; constructor | lia ]);
-    subst; destruct (Equalities.Value_eqb _ _); [inversion H; subst; inversion H1; [ simpl;
-    constructor | lia] | inversion H; subst; inversion H1; [ simpl; constructor | lia] ].
-  * destruct v; try (subst; inversion H3; subst; inversion H1; [subst; simpl; constructor | lia ]);
-    subst; destruct (Equalities.Value_eqb _ _); [inversion H; subst; inversion H1; [ simpl;
-    constructor | lia] | inversion H; subst; inversion H1; [ simpl; constructor | lia] ].
-  * destruct v; try (subst; inversion H3; subst; inversion H1; [subst; simpl; constructor | lia ]);
-    subst; destruct (Equalities.Value_eqb _ _); [inversion H; subst; inversion H1; [ simpl;
-    constructor | lia] | inversion H; subst; inversion H1; [ simpl; constructor | lia] ].
-  * destruct v; try (subst; inversion H3; subst; inversion H1; [subst; simpl; constructor | lia ]);
-    subst; destruct (Equalities.Value_eqb _ _); [inversion H; subst; inversion H1; [ simpl;
-    constructor | lia] | inversion H; subst; inversion H1; [ simpl; constructor | lia] ].
-  * destruct v; try (subst; inversion H3; subst; inversion H1; [subst; simpl; constructor | lia ]);
-    subst; destruct (Equalities.Value_eqb _ _); [inversion H; subst; inversion H1; [ simpl;
-    constructor | lia] | inversion H; subst; inversion H1; [ simpl; constructor | lia] ].
-  * destruct v; try (subst; inversion H3; subst; inversion H1; [subst; simpl; constructor | lia ]);
-    subst; destruct (Equalities.Value_eqb _ _); [inversion H; subst; inversion H1; [ simpl;
-    constructor | lia] | inversion H; subst; inversion H1; [ simpl; constructor | lia] ].
-  * destruct v; try (subst; inversion H3; subst; inversion H1; [subst; simpl; constructor | lia ]);
-    subst; destruct (Equalities.Value_eqb _ _); [inversion H; subst; inversion H1; [ simpl;
-    constructor | lia] | inversion H; subst; inversion H1; [ simpl; constructor | lia] ].
-  * destruct v; try (subst; inversion H3; subst; inversion H1; [subst; simpl; constructor | lia ]).
-  * destruct v; try (subst; inversion H3; subst; inversion H1; [subst; simpl; constructor | lia ]);
-    subst; destruct (Equalities.Value_eqb _ _); [inversion H; subst; inversion H1; [ simpl;
-    constructor | lia] | inversion H; subst; inversion H1; [ simpl; constructor | lia] ].
-  * destruct v; try (subst; inversion H3; subst; inversion H1; [subst; simpl; constructor | lia ]);
-    subst; destruct (Equalities.Value_eqb _ _); [inversion H; subst; inversion H1; [ simpl;
-    constructor | lia] | inversion H; subst; inversion H1; [ simpl; constructor | lia] ].
-  * destruct v; try (subst; inversion H3; subst; inversion H1; [subst; simpl; constructor | lia ]);
-    subst; destruct (Equalities.Value_eqb _ _); [inversion H; subst; inversion H1; [ simpl;
-    constructor | lia] | inversion H; subst; inversion H1; [ simpl; constructor | lia] ].
-  * destruct v; try (subst; inversion H3; subst; inversion H1; [subst; simpl; constructor | lia ]);
-    subst; destruct (Equalities.Value_eqb _ _); [inversion H; subst; inversion H1; [ simpl;
-    constructor | lia] | inversion H; subst; inversion H1; [ simpl; constructor | lia] ].
-  * destruct v; try (subst; inversion H3; subst; inversion H1; [subst; simpl; constructor | lia ]);
-    subst; destruct (Equalities.Value_eqb _ _); [inversion H; subst; inversion H1; [ simpl;
-    constructor | lia] | inversion H; subst; inversion H1; [ simpl; constructor | lia] ].
-  * destruct v; try (subst; inversion H3; subst; inversion H1; [subst; simpl; constructor | lia ]);
-    subst; destruct (Equalities.Value_eqb _ _); [inversion H; subst; inversion H1; [ simpl;
-    constructor | lia] | inversion H; subst; inversion H1; [ simpl; constructor | lia] ].
-  * destruct v; try (subst; inversion H3; subst; inversion H1; [subst; simpl; constructor | lia ]);
-    subst; destruct (Equalities.Value_eqb _ _); [inversion H; subst; inversion H1; [ simpl;
-    constructor | lia] | inversion H; subst; inversion H1; [ simpl; constructor | lia] ].
-  * destruct v; try (subst; inversion H3; subst; inversion H1; [subst; simpl; constructor | lia ]);
-    subst; destruct (Equalities.Value_eqb _ _); [inversion H; subst; inversion H1; [ simpl;
-    constructor | lia] | inversion H; subst; inversion H1; [ simpl; constructor | lia] ].
-  * destruct v; try (subst; inversion H3; subst; inversion H1; [subst; simpl; constructor | lia ]);
-    subst; destruct (Equalities.Value_eqb _ _); [inversion H; subst; inversion H1; [ simpl;
-    constructor | lia] | inversion H; subst; inversion H1; [ simpl; constructor | lia] ].
-  * destruct v; try (subst; inversion H3; subst; inversion H1; [subst; simpl; constructor | lia ]);
-    subst; destruct (Equalities.Value_eqb _ _); [inversion H; subst; inversion H1; [ simpl;
-    constructor | lia] | inversion H; subst; inversion H1; [ simpl; constructor | lia] ].
-  * destruct v; try (subst; inversion H3; subst; inversion H1; [subst; simpl; constructor | lia ]).
-  * destruct v; try (subst; inversion H3; subst; inversion H1; [subst; simpl; constructor | lia ]);
-    subst; destruct (Equalities.Value_eqb _ _); [inversion H; subst; inversion H1; [ simpl;
-    constructor | lia] | inversion H; subst; inversion H1; [ simpl; constructor | lia] ].
-  * destruct v; try (subst; inversion H3; subst; inversion H1; [subst; simpl; constructor | lia ]);
-    subst; destruct (Equalities.Value_eqb _ _); [inversion H; subst; inversion H1; [ simpl;
-    constructor | lia] | inversion H; subst; inversion H1; [ simpl; constructor | lia] ].
-  * destruct v; try (subst; inversion H3; subst; inversion H1; [subst; simpl; constructor | lia ]);
-    subst; destruct (Equalities.Value_eqb _ _); [inversion H; subst; inversion H1; [ simpl;
-    constructor | lia] | inversion H; subst; inversion H1; [ simpl; constructor | lia] ].
-  * destruct v; try (subst; inversion H3; subst; inversion H1; [subst; simpl; constructor | lia ]);
-    subst; destruct (Equalities.Value_eqb _ _); [inversion H; subst; inversion H1; [ simpl;
-    constructor | lia] | inversion H; subst; inversion H1; [ simpl; constructor | lia] ].
-  * destruct v; try (subst; inversion H3; subst; inversion H1; [subst; simpl; constructor | lia ]);
-    subst; destruct (Equalities.Value_eqb _ _); [inversion H; subst; inversion H1; [ simpl;
-    constructor | lia] | inversion H; subst; inversion H1; [ simpl; constructor | lia] ].
-  * destruct v; try (subst; inversion H3; subst; inversion H1; [subst; simpl; constructor | lia ]);
-    subst; destruct (Equalities.Value_eqb _ _); [inversion H; subst; inversion H1; [ simpl;
-    constructor | lia] | inversion H; subst; inversion H1; [ simpl; constructor | lia] ].
-  * destruct v; try (subst; inversion H3; subst; inversion H1; [subst; simpl; constructor | lia ]);
-    subst; destruct (Equalities.Value_eqb _ _); [inversion H; subst; inversion H1; [ simpl;
-    constructor | lia] | inversion H; subst; inversion H1; [ simpl; constructor | lia] ].
-  * destruct v; try (subst; inversion H3; subst; inversion H1; [subst; simpl; constructor | lia ]);
-    subst; destruct (Equalities.Value_eqb _ _); [inversion H; subst; inversion H1; [ simpl;
-    constructor | lia] | inversion H; subst; inversion H1; [ simpl; constructor | lia] ].
-  * destruct v; try (subst; inversion H3; subst; inversion H1; [subst; simpl; constructor | lia ]);
-    subst; destruct (Equalities.Value_eqb _ _); [inversion H; subst; inversion H1; [ simpl;
-    constructor | lia] | inversion H; subst; inversion H1; [ simpl; constructor | lia] ].
-  * destruct v; try (subst; inversion H3; subst; inversion H1; [subst; simpl; constructor | lia ]);
-    subst; destruct (Equalities.Value_eqb _ _); [inversion H; subst; inversion H1; [ simpl;
-    constructor | lia] | inversion H; subst; inversion H1; [ simpl; constructor | lia] ].
-  * subst. admit. (* i=0 but it needs i=1. What to do? *)
-  * subst. admit. (* seem too long too many destructs *)
-  * subst. admit. (* What to do? *) (* destruct eval_subtract _ _ ? *) 
-  * subst. admit.
-  * subst. admit.
-  * subst. admit.
-  * subst. admit.
-  * subst. admit.
-  * subst. admit.
-  * subst. admit.
-  * subst. admit.
-  * subst. admit.
-  * subst. admit.
-  * subst. admit. (* destruct transform_tuple _ ? *) 
-  * subst. admit. (* destruct transform_tuple _ ? *) 
-  * subst. inversion H1.
-    - subst. simpl. constructor. intros. inversion H2.
-    - lia.
-  * destruct (transform_list (VCons v1 v2)); subst; inversion H; subst.
-    - inversion H1.
-      + simpl. constructor. admit. (* where is l ?*)
-      + lia.
-  * subst; destruct (Equalities.Value_ltb _ _); inversion H; subst;
-    try (inversion H1; [simpl; constructor | lia]).
-  * subst; destruct (Equalities.Value_ltb _ _); inversion H; subst;
-    try (inversion H1; [simpl; constructor | lia]).
-  * subst; destruct (Equalities.Value_ltb _ _); inversion H; subst;
-    try (inversion H1; [simpl; constructor | lia]).
-  * subst; destruct (Equalities.Value_ltb _ _); inversion H; subst;
-    try (inversion H1; [simpl; constructor | lia]).
-  * subst; destruct (Equalities.Value_ltb _ _); inversion H; subst;
-    try (inversion H1; [simpl; constructor | lia]).
-  * subst; destruct (Equalities.Value_ltb _ _); inversion H; subst;
-    try (inversion H1; [simpl; constructor | lia]).
-  * subst; destruct (Equalities.Value_ltb _ _); inversion H; subst;
-    try (inversion H1; [simpl; constructor | lia]).
-  * subst; destruct (Equalities.Value_ltb _ _); inversion H; subst;
-    try (inversion H1; [simpl; constructor | lia]).
-  * subst; destruct (Equalities.Value_ltb _ _); inversion H; subst;
-    try (inversion H1; [simpl; constructor | lia]).
-  * subst; destruct (Equalities.Value_ltb _ _); inversion H; subst;
-    try (inversion H1; [simpl; constructor | lia]).
-  * subst; destruct (Equalities.Value_ltb _ _); inversion H; subst;
-    try (inversion H1; [simpl; constructor | lia]).
-  * subst; destruct (Equalities.Value_ltb _ _ || Equalities.Value_eqb _ _)%bool;
-    inversion H; subst; try (inversion H1; [simpl; constructor | lia]).
-  * subst; destruct (Equalities.Value_ltb _ _ || Equalities.Value_eqb _ _)%bool;
-    inversion H; subst; try (inversion H1; [simpl; constructor | lia]).
-  * subst; destruct (Equalities.Value_ltb _ _ || Equalities.Value_eqb _ _)%bool;
-    inversion H; subst; try (inversion H1; [simpl; constructor | lia]).
-  * subst; destruct (Equalities.Value_ltb _ _ || Equalities.Value_eqb _ _)%bool;
-    inversion H; subst; try (inversion H1; [simpl; constructor | lia]).
-  * subst; destruct (Equalities.Value_ltb _ _ || Equalities.Value_eqb _ _)%bool;
-    inversion H; subst; try (inversion H1; [simpl; constructor | lia]).
-  * subst; destruct (Equalities.Value_ltb _ _ || Equalities.Value_eqb _ _)%bool;
-    inversion H; subst; try (inversion H1; [simpl; constructor | lia]).
-  * subst; destruct (Equalities.Value_ltb _ _ || Equalities.Value_eqb _ _)%bool;
-    inversion H; subst; try (inversion H1; [simpl; constructor | lia]).
-  * subst; destruct (Equalities.Value_ltb _ _ || Equalities.Value_eqb _ _)%bool;
-    inversion H; subst; try (inversion H1; [simpl; constructor | lia]).
-  * subst; destruct (Equalities.Value_ltb _ _ || Equalities.Value_eqb _ _)%bool;
-    inversion H; subst; try (inversion H1; [simpl; constructor | lia]).
-  * subst; destruct (Equalities.Value_ltb _ _ || Equalities.Value_eqb _ _)%bool;
-    inversion H; subst; try (inversion H1; [simpl; constructor | lia]).
-  * subst; destruct (Equalities.Value_ltb _ _ || Equalities.Value_eqb _ _)%bool;
-    inversion H; subst; try (inversion H1; [simpl; constructor | lia]).
-  * subst; destruct (Equalities.Value_ltb _ _)%bool;
-    inversion H; subst; try (inversion H1; [simpl; constructor | lia]).
-  * subst; destruct (Equalities.Value_ltb _ _)%bool;
-    inversion H; subst; try (inversion H1; [simpl; constructor | lia]).
-  * subst; destruct (Equalities.Value_ltb _ _)%bool;
-    inversion H; subst; try (inversion H1; [simpl; constructor | lia]).
-  * subst; destruct (Equalities.Value_ltb _ _)%bool;
-    inversion H; subst; try (inversion H1; [simpl; constructor | lia]).
-  * subst; destruct (Equalities.Value_ltb _ _)%bool;
-    inversion H; subst; try (inversion H1; [simpl; constructor | lia]).
-  * subst; destruct (Equalities.Value_ltb _ _)%bool;
-    inversion H; subst; try (inversion H1; [simpl; constructor | lia]).
-  * subst; destruct (Equalities.Value_ltb _ _)%bool;
-    inversion H; subst; try (inversion H1; [simpl; constructor | lia]).
-  * subst; destruct (Equalities.Value_ltb _ _)%bool;
-    inversion H; subst; try (inversion H1; [simpl; constructor | lia]).
-  * subst; destruct (Equalities.Value_ltb _ _)%bool;
-    inversion H; subst; try (inversion H1; [simpl; constructor | lia]).
-  * subst; destruct (Equalities.Value_ltb _ _)%bool;
-    inversion H; subst; try (inversion H1; [simpl; constructor | lia]).
-  * subst; destruct (Equalities.Value_ltb _ _)%bool;
-    inversion H; subst; try (inversion H1; [simpl; constructor | lia]).
-  * subst; destruct (Equalities.Value_ltb _ _ || Equalities.Value_eqb _ _)%bool;
-    inversion H; subst; try (inversion H1; [simpl; constructor | lia]).
-  * subst; destruct (Equalities.Value_ltb _ _ || Equalities.Value_eqb _ _)%bool;
-    inversion H; subst; try (inversion H1; [simpl; constructor | lia]).
-  * subst; destruct (Equalities.Value_ltb _ _ || Equalities.Value_eqb _ _)%bool;
-    inversion H; subst; try (inversion H1; [simpl; constructor | lia]).
-  * subst; destruct (Equalities.Value_ltb _ _ || Equalities.Value_eqb _ _)%bool;
-    inversion H; subst; try (inversion H1; [simpl; constructor | lia]).
-  * subst; destruct (Equalities.Value_ltb _ _ || Equalities.Value_eqb _ _)%bool;
-    inversion H; subst; try (inversion H1; [simpl; constructor | lia]).
-  * subst; destruct (Equalities.Value_ltb _ _ || Equalities.Value_eqb _ _)%bool;
-    inversion H; subst; try (inversion H1; [simpl; constructor | lia]).
-  * subst; destruct (Equalities.Value_ltb _ _ || Equalities.Value_eqb _ _)%bool;
-    inversion H; subst; try (inversion H1; [simpl; constructor | lia]).
-  * subst; destruct (Equalities.Value_ltb _ _ || Equalities.Value_eqb _ _)%bool;
-    inversion H; subst; try (inversion H1; [simpl; constructor | lia]).
-  * subst; destruct (Equalities.Value_ltb _ _ || Equalities.Value_eqb _ _)%bool;
-    inversion H; subst; try (inversion H1; [simpl; constructor | lia]).
-  * subst; destruct (Equalities.Value_ltb _ _ || Equalities.Value_eqb _ _)%bool;
-    inversion H; subst; try (inversion H1; [simpl; constructor | lia]).
-  * subst; destruct (Equalities.Value_ltb _ _ || Equalities.Value_eqb _ _)%bool;
-    inversion H; subst; try (inversion H1; [simpl; constructor | lia]).
-  * subst. inversion H1.
-    - subst. simpl. constructor.
-    - lia.
-  * subst. admit. (* destruct eval_length [VCons v1 v2] ?*)
-  * subst; inversion H1; [subst; simpl; constructor | lia].
-  * subst; inversion H1; [subst; simpl; constructor | lia].
-  * subst. inversion H1.
-    - subst. simpl. specialize (H0 0 ltac:(simpl;lia)). simpl in *.
-      inversion H0. auto.
-    - lia.
-  * subst. inversion H1.
-    - subst. simpl. specialize (H0 0 ltac:(simpl;lia)). simpl in *.
-      inversion H0. auto.
-    - lia.
-  * subst. destruct v; inversion H.
-    - destruct x; inversion H.
-      + destruct (nth_error l (Init.Nat.pred (Pos.to_nat p))); inversion H.
-        ** subst. admit. (*Where is v? *)
-  * subst. destruct v; inversion H.
-  * subst. destruct params; inversion H.
-  * subst. destruct v; inversion H.
-  * subst. destruct params; inversion H.
-  * subst. destruct v; inversion H; subst; destruct params; inversion H.
-    - destruct x; inversion H.
-      + destruct (replace_nth_error l (Init.Nat.pred (Pos.to_nat p)) v0); inversion H.
-        ** subst. inversion H1.
-           -- subst. simpl. constructor.
-              admit. (* Were is l0? *)
-           -- lia.
-  * destruct params; inversion H.
-  * destruct params; inversion H.
-  * destruct params; inversion H.
-  * destruct params; inversion H.
-  * destruct params; inversion H.
-  * destruct params; inversion H.
-  * destruct params; inversion H.
-  * destruct params; inversion H.
-  * subst; inversion H1; [subst; simpl; constructor | lia].
-  * subst; inversion H1; [subst; simpl; constructor | lia].
-  * subst; inversion H1; [subst; simpl; constructor | lia].
-  * subst; inversion H1; [subst; simpl; constructor | lia].
-  * subst; inversion H1; [subst; simpl; constructor | lia].
-  * subst; inversion H1; [subst; simpl; constructor | lia].
-  * subst; inversion H1; [subst; simpl; constructor | lia].
-  * subst; inversion H1; [subst; simpl; constructor | lia].
-  * subst; inversion H1; [subst; simpl; constructor | lia].
-  * subst; inversion H1; [subst; simpl; constructor | lia].
-  * subst; inversion H1; [subst; simpl; constructor | lia].
-  * subst; inversion H1; [subst; simpl; constructor | lia].
-  * subst; inversion H1; [subst; simpl; constructor | lia].
-  * subst; inversion H1; [subst; simpl; constructor | lia].
-  * subst; inversion H1; [subst; simpl; constructor | lia].
-  * subst; inversion H1; [subst; simpl; constructor | lia].
-  * subst; inversion H1; [subst; simpl; constructor | lia].
-  * subst; inversion H1; [subst; simpl; constructor | lia].
-  * subst; inversion H1; [subst; simpl; constructor | lia].
-  * subst; inversion H1; [subst; simpl; constructor | lia].
-  * subst; inversion H1; [subst; simpl; constructor | lia].
-  * subst; inversion H1; [subst; simpl; constructor | lia].
-  * subst; inversion H1; [subst; simpl; constructor | lia].
-  * subst; inversion H1; [subst; simpl; constructor | lia].
-  * subst; inversion H1; [subst; simpl; constructor | lia].
-  * subst; inversion H1; [subst; simpl; constructor | lia].
-  * subst; inversion H1; [subst; simpl; constructor | lia].
-  * subst; inversion H1; [subst; simpl; constructor | lia].
-  * subst; inversion H1; [subst; simpl; constructor | lia].
-  * subst; inversion H1; [subst; simpl; constructor | lia].
-  * subst; inversion H1; [subst; simpl; constructor | lia].
-  * subst; inversion H1; [subst; simpl; constructor | lia].
-  * subst; inversion H1; [subst; simpl; constructor | lia].
-  * subst; inversion H1; [subst; simpl; constructor | lia].
-  * subst; destruct (Equalities.Value_eqb _ _ || Equalities.Value_eqb _ _)%bool;
-    inversion H; subst; try (inversion H1; [simpl; constructor | lia]).
-  * subst; destruct (Equalities.Value_eqb _ _ || Equalities.Value_eqb _ _)%bool;
-    inversion H; subst; try (inversion H1; [simpl; constructor | lia]).
-  * subst; destruct (Equalities.Value_eqb _ _ || Equalities.Value_eqb _ _)%bool;
-    inversion H; subst; try (inversion H1; [simpl; constructor | lia]).
-  * subst; destruct (Equalities.Value_eqb _ _ || Equalities.Value_eqb _ _)%bool;
-    inversion H; subst; try (inversion H1; [simpl; constructor | lia]).
-  * subst; destruct (Equalities.Value_eqb _ _ || Equalities.Value_eqb _ _)%bool;
-    inversion H; subst; try (inversion H1; [simpl; constructor | lia]).
-  * subst; destruct (Equalities.Value_eqb _ _ || Equalities.Value_eqb _ _)%bool;
-    inversion H; subst; try (inversion H1; [simpl; constructor | lia]).
-  * subst; destruct (Equalities.Value_eqb _ _ || Equalities.Value_eqb _ _)%bool;
-    inversion H; subst; try (inversion H1; [simpl; constructor | lia]).
-  * subst; destruct (Equalities.Value_eqb _ _ || Equalities.Value_eqb _ _)%bool;
-    inversion H; subst; try (inversion H1; [simpl; constructor | lia]).
-  * subst; destruct (Equalities.Value_eqb _ _ || Equalities.Value_eqb _ _)%bool;
-    inversion H; subst; try (inversion H1; [simpl; constructor | lia]).
-  * subst; destruct (Equalities.Value_eqb _ _ || Equalities.Value_eqb _ _)%bool;
-    inversion H; subst; try (inversion H1; [simpl; constructor | lia]).
-
-Admitted.
-*)
-
-Theorem convert_to_closlist_keeps_scope :
-  forall ext Γ,
-  (forall i, i < length ext -> 
-  EXP Datatypes.length ext + (nth i (map snd (map fst ext)) 0) + Γ ⊢ nth i (map snd ext) (Val VNil))
-  -> forall i, i < length ext -> VAL Γ ⊢ nth i (convert_to_closlist ext) VNil.
-Proof.
-  unfold convert_to_closlist. induction ext; intros. 
-  * simpl in *. destruct i.
-    - lia.
-    - constructor.
-  * destruct i.
-    - destruct a. destruct p. constructor.
-      + intros. destruct i.
-        ** simpl in *. apply (H 0). lia.
-        ** simpl. simpl in H1.
-           specialize (H (S i) ltac:(simpl;lia)). simpl in H. auto.
-      + simpl. apply (H 0). lia.
-    - assert ((forall i : nat,
-         i < Datatypes.length ext ->
-         EXP Datatypes.length ext +
-             nth i (map snd (map fst ext)) 0 + S Γ
-         ⊢ nth i (map snd ext) (Val VNil))). {
-           intros. Search plus S.  rewrite Nat.add_succ_r. apply (H (S i0)). simpl. lia.
-         }
-         simpl in H0.
-         specialize (IHext _ H1 i ltac:(simpl;lia)). simpl.
-         Search nth.
-         
-Admitted.
-
-
-(* This needs the eval_is_closed Lemma*)
-Theorem step_closedness : forall F p F' p',
-   ⟨ F, p ⟩ --> ⟨ F', p' ⟩ -> FSCLOSED F -> PROGCLOSED p
+Corollary step_term_term :
+  forall k n fs e fs' e',
+  ⟨fs, e⟩ -[k]-> ⟨fs', e'⟩ -> | fs', e' | n - k ↓ -> n >= k 
 ->
-  FSCLOSED F' /\ PROGCLOSED p'.
+  | fs, e | n ↓.
 Proof.
-  intros. inversion H; subst.
-  * inversion H1. subst. split.
-    - auto.
-    - inversion H3. subst. constructor. intros. destruct i.
-      + simpl. auto.
-      + simpl in H2. lia.
-  * inversion H1. subst. split.
-    - auto.
-    - constructor. intros. destruct i.
-      + simpl. constructor.
-      + simpl. constructor.
-  * inversion H1. subst. inversion H0. subst. inversion H5. subst. split.
-    - constructor.
-      + constructor.
-        ** Check indexed_to_forall. rewrite <- (indexed_to_forall _ (fun v => VALCLOSED v) _). Check Forall_app. apply Forall_app. 
-        split.
-           -- rewrite (indexed_to_forall _ _ VNil). auto.
-           -- rewrite (indexed_to_forall _ _ VNil). auto.
-        ** rewrite <- (indexed_to_forall _ (fun e => EXPCLOSED e) _).
-           rewrite <- (indexed_to_forall _ (fun e => EXPCLOSED e) _) in H8.
-           replace (e :: el) with ([e] ++ el) in H8 by (simpl;auto).
-           rewrite Forall_app in H8. destruct H8. auto.
-      + auto.
-    - constructor. specialize (H8 0 ltac:(simpl;lia)). simpl in H8. auto.
-  * inversion H0. subst. clear H0. inversion H1. subst. clear H1. inversion H4. subst.
-    clear H4. split.
-    - auto.
-    - constructor. rewrite <- (indexed_to_forall _ (fun v => VALCLOSED v) _).
-      rewrite <- (indexed_to_forall _ (fun v => VALCLOSED v) _) in H2.
-      rewrite <- (indexed_to_forall _ (fun v => VALCLOSED v) _) in H3.
-      apply Forall_app. auto.
-  * inversion H1. subst. clear H1. inversion H3. subst. clear H3. inversion H2. subst. 
-    clear H2. split.
-    - constructor.
-      + constructor.
-        ** intros. simpl in H1. lia.
-        ** rewrite <- (indexed_to_forall _ (fun e => EXPCLOSED e) _) in H3.
-           rewrite <- (indexed_to_forall _ (fun e => EXPCLOSED e) _).
-           replace (e :: el) with ([e] ++ el) in H3 by (simpl;auto).
-           rewrite Forall_app in H3. destruct H3. auto.
-      + auto.
-    - constructor. specialize (H3 0 ltac:(simpl;lia)). simpl in H3. auto.
-  * inversion H0. subst. clear H0. inversion H1. subst. clear H1. inversion H4. subst.
-    clear H4. split.
-    - constructor. 
-      + constructor. specialize (H2 0 ltac:(simpl;lia)). simpl in H2. auto.
-      + auto.
-    - constructor. auto.
-  * inversion H0. subst. clear H0. inversion H1. subst. clear H1. inversion H4. subst.
-    clear H4. split.
-    - auto.
-    - constructor. intros. simpl in H0. specialize (H2 i ltac:(simpl;lia)).
-      inversion H0.
-      + subst. simpl in *. constructor.
-        ** auto.
-        ** auto.
-      + lia.
-  * inversion H1. subst. clear H1. inversion H3. subst. clear H3. inversion H2. subst.
-    clear H2. split.
-    - constructor.
-      + constructor. auto.
-      + auto.
-    - constructor. auto.
-  * inversion H1. subst. clear H1. inversion H3. subst. clear H3. inversion H2. subst.
-    clear H2. split.
-    - auto.
-    - constructor. intros. destruct i.
-      + simpl. constructor. intros. simpl. destruct i.
-        ** constructor.
-        ** constructor.
-      + simpl in H1. lia.
-  * inversion H0. subst. clear H0. inversion H1. subst. clear H1. inversion H4. subst.
-    clear H4. split.
-    - constructor.
-      + constructor.
-        ** rewrite <- (indexed_to_forall _ (fun v => VALCLOSED v) _).
-           rewrite <- (indexed_to_forall _ (fun v => VALCLOSED v) _) in H2.
-           rewrite <- (indexed_to_forall _ (fun v => VALCLOSED v) _) in H3.
-           apply Forall_app. auto.
-        ** rewrite <- (indexed_to_forall _ (fun e => EXPCLOSED e) _).
-           rewrite <- (indexed_to_forall _ (fun e => EXPCLOSED e) _) in H6.
-           replace (e :: el) with ([e] ++ el) in H6 by (simpl;auto).
-           rewrite Forall_app in H6. destruct H6. auto.
-      + auto.
-    - constructor. rewrite <- (indexed_to_forall _ (fun e => EXPCLOSED e) _) in H6.
-      replace (e :: el) with ([e] ++ el) in H6 by (simpl;auto).
-      rewrite Forall_app in H6. destruct H6. rewrite indexed_to_forall in H0.
-      specialize (H0 0). simpl in H0. apply H0. auto.
-  * inversion H0. subst. clear H0. inversion H1. subst. clear H1. inversion H4. subst.
-    clear H4. split.
-    - auto.
-    - constructor. destruct i.
-      + simpl. intros. constructor.
-        rewrite <- (indexed_to_forall _ (fun v => VALCLOSED v) _).
-        rewrite <- (indexed_to_forall _ (fun v => VALCLOSED v) _) in H2.
-        rewrite <- (indexed_to_forall _ (fun v => VALCLOSED v) _) in H3.
-        apply Forall_app. auto.
-      + simpl. intros. lia.
-  * inversion H1. subst. clear H1. inversion H3. subst. clear H3. inversion H2. subst.
-    clear H2. split.
-    - constructor.
-      + constructor.
-        ** simpl. intros. lia.
-        ** rewrite <- (indexed_to_forall _ (fun e => EXPCLOSED e) _).
-           rewrite <- (indexed_to_forall _ (fun e => EXPCLOSED e) _) in H3.
-           replace (e :: el) with ([e] ++ el) in H3 by (simpl;auto).
-           rewrite Forall_app in H3. destruct H3. auto.
-      + auto.
-    - constructor. rewrite <- (indexed_to_forall _ (fun e => EXPCLOSED e) _) in H3.
-      replace (e :: el) with ([e] ++ el) in H3 by (simpl;auto).
-      rewrite Forall_app in H3. destruct H3. inversion H1. subst. auto.
-  * inversion H1. subst. clear H1. inversion H3. subst. clear H3. inversion H2. subst.
-    clear H2. split.
-    - auto.
-    - constructor. intros. simpl in H1. destruct i.
-      + simpl. constructor. 
-        ** intros. simpl in H2. lia.
-        ** intros. simpl in H2. lia.
-      + lia.
-  * inversion H0. subst. clear H0. inversion H1. subst. clear H1. inversion H4. subst.
-    clear H4. split.
-    - constructor.
-      + constructor.
-        ** auto.
-        ** auto.
-        ** auto.
-        ** auto.
-        ** specialize (H2 0). simpl in H2. apply H2. auto.
-      + auto.
-    - constructor. auto.
-  * inversion H0. subst. clear H0. inversion H1. subst. clear H1. inversion H4. subst.
-    clear H4. split.
-    - assert (forall i, i < length vl -> VALCLOSED (fst (nth i vl (VNil, VNil)))) as H11.
-      { clear H H2 H5 H7 H8 H9 H10. intros. specialize (H6 i H).
-        replace VNil with (fst (VNil, VNil)) in H6 by auto.
-        rewrite map_nth in H6. auto. } (* prooving the assert is correct based on H6 *)
-      clear H6. rewrite <- (indexed_to_forall _ (fun v => VALCLOSED (fst v)) _) in H11.
-      
-      assert (forall i, i < length vl -> VALCLOSED (snd (nth i vl (VNil, VNil)))) as H12.
-      { clear H H2 H5 H8 H9 H10. intros. specialize (H7 i H).
-        replace VNil with (snd (VNil, VNil)) in H7 by auto.
-        rewrite map_nth in H7. auto. } (* prooving the assert is correct based on H7 *)
-      clear H7. rewrite <- (indexed_to_forall _ (fun v => VALCLOSED (snd v)) _) in H12.
-      
-      specialize (H2 0 ltac:(simpl;lia)). simpl in H2.
-      
-      assert (forall i, i < length ((fs', sn') :: el) -> 
-      EXPCLOSED (fst (nth i ((fs', sn') :: el) (Val VNil, Val VNil)))) as H13.
-      { intros. specialize (H8 i H0). replace (Val VNil) with (fst (Val VNil, Val VNil))
-        in H8 by auto. rewrite map_nth in H8. auto. }
-      clear H8. rewrite <- (indexed_to_forall _ (fun e => EXPCLOSED (fst e)) _) in H13.
-      
-      assert (forall i, i < length ((fs', sn') :: el) -> 
-      EXPCLOSED (snd (nth i ((fs', sn') :: el) (Val VNil, Val VNil)))) as H14.
-      { intros. specialize (H9 i H0). replace (Val VNil) with (snd (Val VNil, Val VNil))
-        in H9 by auto. rewrite map_nth in H9. auto. }
-      clear H9. rewrite <- (indexed_to_forall _ (fun e => EXPCLOSED (snd e)) _) in H14.
-      
-      replace ((fs', sn') :: el) with ([(fs', sn')] ++ el) in H13 by (simpl;auto).
-      replace ((fs', sn') :: el) with ([(fs', sn')] ++ el) in H14 by (simpl;auto).
-      rewrite Forall_app in H13. destruct H13. rewrite Forall_app in H14. destruct H14.
-      
-      constructor.
-      
-      + constructor.
-        ** intros. replace VNil with (fst (VNil,VNil)) by auto.
-           rewrite map_nth. revert H6. revert i.
-           rewrite <- (indexed_to_forall _ (fun v => VALCLOSED (fst v)) _).
-           apply Forall_app. split.
-           -- auto.
-           -- constructor.
-              ++ auto.
-              ++ auto.
-        ** intros. replace VNil with (snd (VNil,VNil)) by auto.
-           rewrite map_nth. revert H6. revert i.
-           rewrite <- (indexed_to_forall _ (fun v => VALCLOSED (snd v)) _).
-           apply Forall_app. split.
-           -- auto.
-           -- constructor.
-              ++ auto.
-              ++ auto.
-        ** intros. replace (Val VNil) with (fst (Val VNil, Val VNil)) by auto.
-           rewrite map_nth. revert H6. revert i.
-           rewrite <- (indexed_to_forall _ (fun e => EXPCLOSED (fst e)) _). auto.
-        ** intros. replace (Val VNil) with (snd (Val VNil, Val VNil)) by auto.
-           rewrite map_nth. revert H6. revert i.
-           rewrite <- (indexed_to_forall _ (fun e => EXPCLOSED (snd e)) _). auto.
-        ** inversion H3. subst. simpl in H8. auto.
-      + auto.
-    - constructor. specialize (H8 0 ltac:(simpl;lia)). simpl in H8. auto.
-  * inversion H0. subst. clear H0. inversion H1. subst. clear H1. inversion H4. subst.
-    clear H4. split.
-    - auto.
-    - constructor. intros. simpl in H0. destruct i.
-      + simpl.
-        
-        assert (forall i, i < length vl -> VALCLOSED (fst (nth i vl (VNil, VNil)))) as H11.
-        { intros. specialize (H6 i H1).
-          replace VNil with (fst (VNil, VNil)) in H6 by auto.
-          rewrite map_nth in H6. auto. } (* prooving the assert is correct based on H6 *)
-        clear H6. rewrite <- (indexed_to_forall _ (fun v => VALCLOSED (fst v)) _) in H11.
-        
-        assert (forall i, i < length vl -> VALCLOSED (snd (nth i vl (VNil, VNil)))) as H12.
-        { intros. specialize (H7 i H1).
-          replace VNil with (snd (VNil, VNil)) in H7 by auto.
-          rewrite map_nth in H7. auto. } (* prooving the assert is correct based on H7 *)
-        clear H7. rewrite <- (indexed_to_forall _ (fun v => VALCLOSED (snd v)) _) in H12.
-        
-        constructor.
-        ** intros. replace VNil with (fst (VNil,VNil)) by auto.
-           rewrite map_nth. revert H1. revert i.
-           rewrite <- (indexed_to_forall _ (fun v => VALCLOSED (fst v)) _).
-           rewrite Forall_app. split.
-           -- auto.
-           -- constructor.
-              ++ simpl. auto.
-              ++ auto.
-        ** intros. replace VNil with (snd (VNil,VNil)) by auto.
-           rewrite map_nth. revert H1. revert i.
-           rewrite <- (indexed_to_forall _ (fun v => VALCLOSED (snd v)) _).
-           rewrite Forall_app. split.
-           -- auto.
-           -- constructor.
-              ++ simpl. specialize (H2 0 ltac:(simpl;lia)). simpl in H2. auto.
-              ++ auto.
-      + lia.
-  * inversion H1. subst. clear H1. inversion H3. subst. clear H3. inversion H2. subst.
-    clear H2. split.
-    - constructor.
-      + constructor.
-        ** intros. simpl. destruct i.
-           -- constructor.
-           -- constructor.
-        ** intros. simpl. destruct i.
-           -- constructor.
-           -- constructor.
-        ** replace (Datatypes.length ((fs, sn) :: el)) with
-           (Datatypes.length (map fst ((fs, sn) :: el))) in H3 by
-           (simpl;rewrite map_length; auto).
-           rewrite <- (indexed_to_forall _ (fun e => EXPCLOSED e) _) in H3.
-           
-           replace (Datatypes.length el) with (Datatypes.length (map fst el)) by
-           (simpl;rewrite map_length; auto).
-           rewrite <- (indexed_to_forall _ (fun e => EXPCLOSED e) _).
-           
-           (* Here this replace was a trickier step. *)
-           replace (map fst ((fs, sn) :: el)) with ([fst (fs, sn)]++(map fst el)) in H3
-           by (simpl;auto). apply Forall_app in H3. destruct H3. auto.
-           
-        ** clear H3. replace (Datatypes.length ((fs, sn) :: el)) with 
-           (Datatypes.length (map snd ((fs, sn) :: el))) in H4 by
-           (simpl;rewrite map_length; auto).
-           rewrite <- (indexed_to_forall _ (fun e => EXPCLOSED e) _) in H4.
-           
-           replace (Datatypes.length el) with (Datatypes.length (map snd el)) by
-           (simpl;rewrite map_length; auto).
-           rewrite <- (indexed_to_forall _ (fun e => EXPCLOSED e) _).
-           
-           replace (map snd ((fs, sn) :: el)) with ([snd (fs, sn)]++(map snd el)) in H4
-           by (simpl;auto). apply Forall_app in H4. destruct H4. auto.
-        
-        ** clear H3. replace (Datatypes.length ((fs, sn) :: el)) with 
-           (Datatypes.length (map snd ((fs, sn) :: el))) in H4 by
-           (simpl;rewrite map_length; auto).
-           rewrite <- (indexed_to_forall _ (fun e => EXPCLOSED e) _) in H4.
-           
-           replace (map snd ((fs, sn) :: el)) with ([snd (fs, sn)]++(map snd el)) in H4
-           by (simpl;auto). apply Forall_app in H4. destruct H4. simpl in H1.
-           inversion H1. subst. auto.
-      + auto.
-    - constructor. replace (Datatypes.length ((fs, sn) :: el)) with
-      (Datatypes.length (map fst ((fs, sn) :: el))) in H3 by
-      (simpl;rewrite map_length; auto).
-      rewrite <- (indexed_to_forall _ (fun e => EXPCLOSED e) _) in H3.
-      
-      replace (map fst ((fs, sn) :: el)) with ([fst (fs, sn)]++(map fst el)) in H3
-      by (simpl;auto). apply Forall_app in H3. destruct H3. simpl in H1.
-      inversion H1. subst. auto.
-  * inversion H1. subst. clear H1. inversion H4. subst. clear H4. inversion H3. subst.
-    clear H3. split.
-    - auto.
-    - admit. (* unclear because of the eval *)
-  * inversion H0. subst. clear H0. inversion H1. subst. clear H1. inversion H4. subst.
-    clear H4. split.
-    - constructor.
-      + constructor.
-        ** rewrite <- (indexed_to_forall _ (fun v => VALCLOSED v) _).
-           rewrite <- (indexed_to_forall _ (fun v => VALCLOSED v) _) in H2.
-           rewrite <- (indexed_to_forall _ (fun v => VALCLOSED v) _) in H3.
-           rewrite Forall_app. auto.
-        ** rewrite <- (indexed_to_forall _ (fun e => EXPCLOSED e) _) in H7.
-           replace (e :: el) with ([e] ++ el) in H7 by (simpl;auto).
-           rewrite Forall_app in H7. destruct H7.
-           rewrite <- (indexed_to_forall _ (fun e => EXPCLOSED e) _). auto.
-      + auto.
-    - rewrite <- (indexed_to_forall _ (fun e => EXPCLOSED e) _) in H7.
-      replace (e :: el) with ([e] ++ el) in H7 by (simpl;auto).
-      rewrite Forall_app in H7. destruct H7. inversion H0. subst. constructor. auto.
-  * inversion H0. subst. clear H0. inversion H1. subst. clear H1. inversion H5. subst.
-    clear H5. split.
-    - auto.
-    - admit. (* unclear because of the eval *)
-  * inversion H1. subst. clear H1. inversion H3. subst. clear H3. inversion H2. subst.
-    clear H2. rewrite <- (indexed_to_forall _ (fun e => EXPCLOSED e) _) in H5.
-    replace (e :: el) with ([e] ++ el) in H5 by (simpl;auto).
-    rewrite Forall_app in H5. destruct H5. split.
-    - constructor.
-      + constructor. 
-        ** intros. simpl in H3. lia.
-        ** rewrite <- (indexed_to_forall _ (fun e => EXPCLOSED e) _). auto.
-      + auto.
-    - constructor. inversion H1. subst. auto.
-  * inversion H1. subst. clear H1. inversion H4. subst. clear H4. inversion H3. subst.
-    clear H3. split.
-    - auto.
-    - destruct exc. destruct p. constructor.
-      + admit. (* unclear because of the eval *)
-      + admit. (* unclear because of the eval *)
-  * inversion H0. subst. clear H0. inversion H1. subst. clear H1. inversion H2. subst.
-    clear H2. inversion H5. subst. clear H5. split.
-    - auto.
-    - destruct exc. destruct p. constructor.
-      + admit. (* unclear because of the eval *)
-      + admit. (* unclear because of the eval *)
-  * inversion H0. subst. clear H0. inversion H1. subst. clear H1. inversion H4. subst.
-    clear H4. split.
-    - auto.
-    - constructor. Search subscoped list_subst.
-      Search subst ExpScoped. apply (subst_preserves_scope_exp _ (length vs)). (* subst is closed, solved*)
-      + auto.
-      + Search subscoped list_subst. apply scoped_list_idsubst. 
-        rewrite -> (indexed_to_forall _ (fun v => VALCLOSED v) VNil). auto.
-  * inversion H1. subst. clear H1. inversion H3. subst. clear H3. inversion H2. subst.
-    clear H2. split.
-    - constructor. 
-      + constructor. replace (l + 0) with l in H7 by auto. auto.
-      + auto.
-    - constructor. auto.
-  * inversion H0. subst. clear H0. inversion H1. subst. clear H1. inversion H4. subst.
-    clear H4. split.
-    - auto.
-    - constructor. auto.
-  * inversion H1. subst. clear H1. inversion H3. subst. clear H3. inversion H2. subst.
-    clear H2. split.
-    - constructor. 
-      + constructor. auto.
-      + auto.
-    - constructor. auto.
-  * inversion H1. subst. clear H1. inversion H3. subst. clear H3. inversion H2. subst.
-    clear H2. split.
-    - auto.
-    - constructor. intros. simpl in H1. inversion H1.
-      + subst. simpl. constructor.
-        ** intros. simpl in H2. lia.
-        ** simpl. auto.
-      + lia.
-  * inversion H1. subst. clear H1. inversion H4. subst. clear H4. inversion H3. subst.
-    clear H3. split.
-    - auto.
-    - admit. (* unclear because of the eval *)
-  * inversion H0. subst. clear H0. inversion H1. subst. clear H1. inversion H4. subst.
-    clear H4.
-    rewrite <- (indexed_to_forall _ (fun v => VALCLOSED v) _) in H2.
-    rewrite <- (indexed_to_forall _ (fun v => VALCLOSED v) _) in H3.
-    rewrite <- (indexed_to_forall _ (fun e => EXPCLOSED e) _) in H7.
-    replace (e :: el) with ([e] ++ el) in H7 by (simpl;auto).
-    rewrite Forall_app in H7. destruct H7. inversion H2. subst. split.
-    - constructor.
-      + constructor.
-        ** rewrite <- (indexed_to_forall _ (fun v => VALCLOSED v) _).
-           rewrite Forall_app. auto.
-        ** rewrite <- (indexed_to_forall _ (fun e => EXPCLOSED e) _). auto.
-      + auto.
-    - constructor. inversion H0. subst. auto.
-  * inversion H0. subst. clear H0. inversion H1. subst. clear H1. inversion H5. subst.
-    clear H5. split.
-    - auto.
-    - admit. (* unclear because of the eval *)
-  * inversion H1. subst. clear H1. inversion H3. subst. clear H3. inversion H2. subst.
-    clear H2.
-    rewrite <- (indexed_to_forall _ (fun e => EXPCLOSED e) _) in H5.
-    replace (e :: el) with ([e] ++ el) in H5 by (simpl;auto).
-    rewrite Forall_app in H5. destruct H5. split.
-    - constructor.
-      + constructor.
-        ** intros. simpl in H3. lia.
-        ** rewrite <- (indexed_to_forall _ (fun e => EXPCLOSED e) _). auto.
-      + auto.
-    - constructor. inversion H1. subst. auto.
-  * inversion H1. subst. clear H1. inversion H4. subst. clear H4. inversion H3. subst.
-    clear H3. split.
-    - auto.
-    - admit. (* unclear because of the eval *)
-  * inversion H0. subst. clear H0. inversion H1. subst. clear H1. inversion H5. subst.
-    clear H5. split.
-    - auto.
-    - destruct exc. destruct p. constructor.
-      + admit. (* unclear because of the eval *)
-      + admit. (* unclear because of the eval *)
-  * inversion H0. subst. clear H0. inversion H1. subst. clear H1. inversion H4. subst.
-    clear H4. split.
-    - auto.
-    - constructor. admit. (* subst is closed theorem needed. *) (* convert_to_closlist *)
-  * inversion H0. subst. clear H0. inversion H1. subst. clear H1. inversion H4. subst.
-    clear H4.
-    rewrite <- (indexed_to_forall _ (fun e => EXPCLOSED e) _) in H1.
-    replace (e :: el) with ([e] ++ el) in H1 by (simpl;auto).
-    rewrite Forall_app in H1. destruct H1. split.
-    - constructor.
-      + constructor.
-        ** intros. simpl in H3. lia.
-        ** rewrite <- (indexed_to_forall _ (fun e => EXPCLOSED e) _). auto.
-        ** specialize (H2 0). simpl in H2. apply H2. auto.
-      + auto.
-    - constructor.  inversion H0. subst. auto.
-  * inversion H1. subst. clear H1. inversion H0. subst. clear H0. inversion H4. subst.
-    clear H4.
-    rewrite <- (indexed_to_forall _ (fun v => VALCLOSED v) _) in H3.
-    rewrite <- (indexed_to_forall _ (fun v => VALCLOSED v) _) in H6.
-    rewrite <- (indexed_to_forall _ (fun e => EXPCLOSED e) _) in H7.
-    replace (e :: el) with ([e] ++ el) in H7 by (simpl;auto). rewrite Forall_app in H7.
-    destruct H7. split.
-    - constructor.
-      + constructor.
-        ** rewrite <- (indexed_to_forall _ (fun v => VALCLOSED v) _).
-           rewrite Forall_app. auto.
-        ** rewrite <- (indexed_to_forall _ (fun e => EXPCLOSED e) _). auto.
-        ** auto.
-      + auto.
-    - constructor. inversion H0. subst. auto.
-  * inversion H0. subst. clear H0. inversion H1. subst. clear H1. inversion H4. subst.
-    clear H4. inversion H8. subst. clear H8. split.
-    - auto.
-    - constructor. Search subscoped list_subst.
-      Search subst ExpScoped. apply (subst_preserves_scope_exp _ (Datatypes.length 
-      (convert_to_closlist ext ++ vl ++ [v]))).
-      + replace (Datatypes.length ext + (Datatypes.length vl + 1) + 0) with 
-        (Datatypes.length (convert_to_closlist ext ++ vl ++ [v])) in H11.
-        ** auto.
-        ** clear. Search length. rewrite app_length. rewrite app_length. simpl.
-           replace (Datatypes.length (convert_to_closlist ext)) with (Datatypes.length ext).
-           -- auto.
-           -- destruct ext.
-              ++ simpl. auto.
-              ++ simpl. rewrite map_length. auto.
-      + Search subscoped list_subst. apply scoped_list_idsubst. rewrite Forall_app. split.
-        ** rewrite -> (indexed_to_forall _ (fun v => VALCLOSED v) VNil).
-           intros. specialize (H10 i). replace (Datatypes.length (convert_to_closlist ext)) with
-           (Datatypes.length ext) in H0.
-           -- clear H H5 H2 H6 H7 H11. specialize (H10 H0). unfold convert_to_closlist.
-              admit. (* I do not see how this *) (* convert_to_closlist *)
-           -- destruct ext.
-              ++ simpl. auto.
-              ++ simpl. rewrite map_length. auto.
-           (* Might need a help teorem abaut: length convert_to_closlist ext = length ext *)
-        ** rewrite Forall_app. split.
-           -- rewrite -> (indexed_to_forall _ (fun v => VALCLOSED v) VNil). auto.
-           -- rewrite -> (indexed_to_forall _ (fun v => VALCLOSED v) VNil). auto.
-        (* subst is closed theorem needed. *)
-  * inversion H1. subst. clear H1. inversion H3. subst. clear H3. inversion H2. subst.
-    clear H2. split.
-    - constructor.
-      + constructor. auto.
-      + auto.
-    - constructor. auto.
-  * inversion H0. subst. clear H0. inversion H1. subst. clear H1. inversion H5. subst.
-    clear H5. split.
-    - auto.
-    - constructor.
-      + constructor.
-      + apply (H3 0 ltac:(simpl;lia)).
-  * inversion H0. subst. clear H0. inversion H1. subst. clear H1. inversion H5. subst.
-    clear H5. inversion H9. subst. clear H9. split.
-    - auto.
-    - constructor.
-      + constructor.
-      + constructor.
-        ** auto.
-        ** auto.
-  * inversion H0. subst. clear H0. inversion H1. subst. clear H1. inversion H5. subst.
-    clear H5. split.
-    - auto.
-    - constructor.
-      + constructor.
-      + specialize (H3 0). simpl in H3. apply H3. auto.
-  * inversion H0. subst. clear H0. inversion H1. subst. clear H1. inversion H5. subst.
-    clear H5. split.
-    - auto.
-    - constructor.
-      + constructor.
-      + auto.
-  * inversion H0. subst. clear H0. inversion H1. subst. clear H1. inversion H5. subst.
-    clear H5. split.
-    - constructor.
-      + constructor.
-        ** intros. apply (H1 (S i)). simpl. lia.
-        ** intros. apply (H4 (S i)). simpl. lia.
-        ** auto.
-        ** admit. (* forall ... VALCLOSED vs -> match_pattern_list lp vs = Some vs' -> forall ... VALCLOSED vs', Something like this is needed here. *)
-        ** clear H1 H3 H6 H2 H. specialize (H4 0 ltac:(simpl;lia)). simpl in H4. auto.
-      + auto.
-    - constructor. admit. (* subst is closed theorem needed. *) 
-  * inversion H0. subst. clear H0. inversion H1. subst. clear H1. inversion H5. subst.
-    clear H5. split.
-    - constructor.
-      + constructor.
-        ** intros. apply (H1 (S i)). simpl. lia.
-        ** intros. apply (H4 (S i)). simpl. lia.
-      + auto.
-    - constructor. auto.
-  * inversion H0. subst. clear H0. inversion H1. subst. clear H1. inversion H4. subst.
-    clear H4. split.
-    - auto.
-    (* - constructor. apply (subst_preserves_scope_exp _ (patternListScope lp)).
-      + auto.
-      + Search subscoped list_subst. apply scoped_list_idsubst. *)
-    - constructor. admit. (* subst is closed theorem needed. *)
-  * inversion H0. subst. clear H0. inversion H1. subst. clear H1. inversion H4. subst.
-    clear H4. split.
-    - constructor. 
-      + constructor.
-        ** auto.
-        ** auto.
-      + auto.
-    - constructor. auto.
-  * inversion H1. subst. clear H1. inversion H3. subst. clear H3. inversion H2. subst.
-    clear H2. split.
-    - constructor.
-      + constructor.
-        ** clear H H0 H4 H7. intros. specialize (H5 i H).
-           replace (patternListScope (nth i (map fst (map fst l)) []) + 0) with 
-           (patternListScope (nth i (map fst (map fst l)) [])) in H5 by (simpl;auto).
-           auto.
-        ** clear H H0 H4 H5. intros. specialize (H7 i H).
-           replace (patternListScope (nth i (map fst (map fst l)) []) + 0) with
-           (patternListScope (nth i (map fst (map fst l)) [])) in H7 by (simpl;auto).
-           auto.
-      + auto.
-    - constructor. auto.
-  * inversion H0. subst. clear H0. inversion H4. subst. clear H4. split.
-    - auto.
-    - constructor.
-      + constructor.
-      + constructor.
-  * inversion H1. subst. clear H1. inversion H3. subst. clear H3. inversion H2. subst.
-    clear H2. split.
-    - auto.
-    (* - constructor. apply (subst_preserves_scope_exp _ (Datatypes.length l + 0)).
-      + auto.
-      + replace (Datatypes.length l + 0) with (Datatypes.length l) by auto.
-        Search subscoped list_subst.
-        remember (convert_to_closlist (map (fun '(x, y) => (0, x, y)) l)) as ls.
-        replace (Datatypes.length l) with (Datatypes.length ls).
-        ** apply scoped_list_idsubst.
-           rewrite -> (indexed_to_forall _ (fun v => VALCLOSED v) VNil).
-           subst. admit.
-        ** subst. destruct l.
-           -- auto.
-           -- simpl. *)
-    - constructor. admit. (* subst is closed theorem needed. *)
-  * inversion H0. subst. clear H0. inversion H1. subst. clear H1. inversion H4. subst.
-    clear H4. split.
-    - auto.
-    - constructor. apply (subst_preserves_scope_exp _ (Datatypes.length vs)).
-      + auto.
-      + apply scoped_list_idsubst. 
-        rewrite -> (indexed_to_forall _ (fun v => VALCLOSED v) VNil). auto.
-  * inversion H0. subst. clear H0. inversion H1. subst. clear H1. inversion H4. subst.
-    clear H4. split.
-    - auto.
-    (*- constructor. apply (subst_preserves_scope_exp _ (3)).
-      + auto.
-      + simpl. *)
-    - constructor. admit. (* subst is closed theorem needed. *)
-  * inversion H1. subst. clear H1. inversion H3. subst. clear H3. inversion H2. subst.
-    clear H2. split.
-    - constructor.
-      + constructor.
-        ** replace (vl1 + 0) with vl1 in H9 by auto. auto.
-        ** replace (vl2 + 0) with vl2 in H10 by auto. auto.
-      + auto.
-    - constructor. auto.
-  * inversion H0. subst. clear H0. inversion H1. subst. clear H1. split.
-    - auto.
-    - constructor.
-      + auto.
-      + auto.
-Admitted.
+  intros. apply terminates_in_k_eq_terminates_in_k_sem.
+  apply terminates_in_k_eq_terminates_in_k_sem in H0. destruct H0, H0.
+  pose proof (transitive_eval H H2). replace (k+(n-k)) with n in H3 by lia.
+  eexists. eauto.
+Qed.
 
-
-
-Theorem result_VALCLOSED_any (fs : FrameStack) (e v : ProgResult) :
-  ⟨ fs, e ⟩ -->* v -> PROGCLOSED v.
-Proof.
-  intros. destruct H.
-  * destruct H. destruct H. destruct H. subst. constructor.
-    intros. inversion H0.
-    - subst. admit.
-    - subst. admit.
-  * admit.
-Admitted.
-
-Corollary step_any_closedness : forall F p v,
-   ⟨ F, p ⟩ -->* v -> FSCLOSED F -> PROGCLOSED p
+Corollary step_term_term_plus :
+  forall k k2 fs e fs' e', 
+  ⟨fs, e⟩ -[k]-> ⟨fs', e'⟩ -> | fs', e' | k2 ↓
 ->
-  PROGCLOSED v.
+  | fs, e | k + k2 ↓.
 Proof.
-  intros. destruct v.
-  * inversion H1.
-    - subst. inversion H.
-      + destruct H3. destruct H3. destruct H3.
-Admitted.
+  intros. apply terminates_in_k_eq_terminates_in_k_sem.
+  apply terminates_in_k_eq_terminates_in_k_sem in H0. destruct H0, H0.
+  pose proof (transitive_eval H H1).
+  eexists. eauto.
+Qed.
 
+Theorem transitive_eval_rev : forall Fs Fs' e e' k1,
+  ⟨ Fs, e ⟩ -[k1]-> ⟨ Fs', e' ⟩-> 
+  forall Fs'' e'' k2,
+  ⟨ Fs, e ⟩ -[k1 + k2]-> ⟨ Fs'', e'' ⟩
+->
+  ⟨ Fs', e' ⟩ -[k2]-> ⟨ Fs'', e'' ⟩.
+Proof.
+  intros Fs Fs' e e' k1 IH. induction IH; intros.
+  * simpl in H. auto.
+  * simpl in H0. inversion H0; subst. eapply step_determinism in H.
+    2: exact H2. destruct H; subst.
+    apply IHIH in H5. auto.
+Qed.
+
+Theorem frame_indep_step : forall e F F' Fs e',
+  ⟨ F :: Fs, e ⟩ --> ⟨ F' :: Fs, e' ⟩
+->
+  forall Fs', ⟨ F :: Fs', e ⟩ --> ⟨ F' :: Fs', e' ⟩.
+Proof.
+  intros. revert Fs'. dependent induction H; intros.
+  all: try constructor; auto.
+  all: try (apply cons_neq in x; contradiction).
+  all: symmetry in x; try (apply cons_neq in x; contradiction).
+Qed.
+
+Theorem frame_indep_red : forall e F Fs e',
+  ⟨ F :: Fs, e ⟩ --> ⟨ Fs, e' ⟩
+->
+  forall Fs', ⟨ F :: Fs', e ⟩ --> ⟨ Fs', e' ⟩.
+Proof.
+  intros. revert Fs'. dependent induction H; intros.
+  all: try constructor; auto.
+  all: try (apply cons_neq in x; contradiction).
+  all: symmetry in x; try (apply cons_cons_neq in x; contradiction).
+Qed.
+
+Theorem frame_indep_core : forall k e Fs Fs' v,
+  ⟨ Fs, e ⟩ -[k]-> ⟨ Fs', v ⟩
+->
+  forall Fs'', ⟨ Fs ++ Fs'', e ⟩ -[k]-> ⟨ Fs' ++ Fs'', v ⟩.
+Proof.
+  induction k; intros.
+  * inversion H. subst. constructor.
+  * inv H. inv H1.
+    all: try now (simpl; econstructor; try constructor; auto).
+    all: try (eapply IHk in H4; simpl in *; econstructor; [constructor | exact H4]); auto.
+Qed.
+
+Theorem frame_indep_nil : forall k e Fs v,
+  ⟨ Fs, e ⟩ -[k]-> ⟨ [], v ⟩
+->
+  forall Fs', ⟨ Fs ++ Fs', e ⟩ -[k]-> ⟨ Fs', v ⟩.
+Proof.
+  intros. eapply frame_indep_core in H. exact H.
+Qed.
+
+#[global]
+Hint Constructors is_result : core.
+
+(* Lemma params_termination :
+  (forall m : nat,
+  m < k ->
+  forall (Fs : FrameStack) (e : Redex),
+  | Fs, e | m ↓ ->
+  e <> RBox ->
+  exists (res : Redex) (k : nat),
+    is_result res /\ ⟨ [], e ⟩ -[ k ]-> ⟨ [], res ⟩) ->
+  | FParams ident vl el :: Fs, v | x ↓
+->
+  ⟨ FParams ident vl (vals ++ e::el) :: Fs, v ⟩ -[a]->
+  ⟨ FParams ident (vl ++ vals) el, e ⟩.
+Proof.
+
+Qed. *)
 (*
-Theorem step_closedness : forall F e F' e',
-   ⟨ F, e ⟩ --> ⟨ F', e' ⟩ -> FSCLOSED F -> EXPCLOSED e
-->
-  FSCLOSED F' /\ EXPCLOSED e'.
+(* NOTE: This is not a duplicate! Do not remove! *)
+Theorem term_eval_empty : forall x Fs e,
+  | Fs, e | x ↓ ->
+  e <> RBox ->
+  exists res k, is_result res /\ ⟨ [], e ⟩ -[k]-> ⟨ [], res ⟩ (* /\ k <= x *).
 Proof.
-  intros F e F' e' IH. induction IH; intros.
-  * inversion H0. subst. inversion H4. inversion H3. subst. split; auto.
-    constructor; auto. constructor; auto.
-  * inversion H. inversion H0. subst. split; auto. inversion H5. subst. cbn in H2.
+  induction x using Wf_nat.lt_wf_ind. destruct x; intros; inversion H0; subst; try congruence.
+  all: try now (exists (RValSeq [v]), 0; split; [ auto | now constructor ]).
+  * exists e, 0. now repeat constructor.
+  * exists (RValSeq [v]), 1. split; [ constructor | do 2 econstructor ].
+  * (* problematic because next step is to reduce RBox! Further case
+       separation is needed! *)
+    inv H5.
+    - apply H in H8 as H8'. destruct H8' as [res [k0 [Hres Hd]]].
+      2: lia. 2: congruence.
+      inv Hres. (* exception is the result or not *)
+      + exists ex, (2 + (k0 + 1)). split; auto.
+        do 2 econstructor. constructor.
+        eapply frame_indep_nil in Hd.
+        eapply transitive_eval. exact Hd.
+        econstructor. constructor. intros. congruence. constructor.
+      + eapply frame_indep_nil in Hd. eapply term_step_term in H8.
+        2: exact Hd. simpl in *.
+        
+  * exists e, 0. split; [ auto | now constructor ].
+  * exists e, 0. split; [ auto | now constructor ].
+  * exists (EFun [] e0), 0. inversion P. split; [ auto | do 2 constructor].
+  * exists e, 0. split; [ auto | now constructor].
+  * exists e, 0. split; [ auto | now constructor ].
+  * exists (ELit i2), 0. split; [ auto | now constructor ].
+  * exists e, 0. split; [ auto | now constructor ].
+  * exists e, 0. split; [ auto | now constructor ].
+  * exists e, 0. split; [ auto | now constructor ].
+  * apply H in H4 as HH. destruct HH, H1, H1. 2: lia.
+    eapply frame_indep_nil in H2 as H2_1.
+    eapply (terminates_step_any_2 _ _ _ _ H4) in H2_1 as H2'.
+    inversion H2'; subst; try inversion_is_value.
+    - apply H in H12. 2: lia. destruct H12, H3, H3.
+      exists x2, (S (x1 + S x3)). split. auto.
+      econstructor. constructor. eapply transitive_eval; eauto.
+      eapply frame_indep_nil in H2. exact H2.
+      econstructor. constructor. all: eauto. inversion P. 2: inversion_is_value.
+      subst. apply -> subst_preserves_scope_exp. exact H13.
+      rewrite (match_pattern_length _ _ _ H11), Nat.add_0_r.
+      eapply scoped_list_idsubst, match_pattern_scoped. exact H9. eauto.
+    - apply H in H12. 2: lia. destruct H12, H3, H3.
+      exists x2, (S (x1 + S x3)). split. auto.
+      econstructor. constructor. eapply transitive_eval; eauto.
+      eapply frame_indep_nil in H2. exact H2.
+      econstructor. apply red_case_false; auto. auto. now inversion P.
+    - now inversion P.
+  * apply H in H4 as v_eval. 2: lia. destruct v_eval, H1, H1.
+    eapply frame_indep_nil in H2 as H2_1.
+    eapply (terminates_step_any_2 _ _ _ _ H4) in H2_1 as H2'.
+    destruct vs.
+    - inversion H2'; subst; try inversion_is_value.
+      apply H in H7. 2: lia. destruct H7, H3, H3.
+      exists x0, (S (x1 + S x2)). split; auto.
+      econstructor. constructor. eapply transitive_eval; eauto.
+      eapply frame_indep_nil in H2. exact H2.
+      econstructor. constructor. auto.
+      inversion H1. apply -> subst_preserves_scope_exp; eauto.
+    - inversion H2'; subst; try inversion_is_value.
+      assert (| FApp2 x0 vs [] :: Fs, e | k ↓) as PP by auto.
+      eapply H in H10. 2: lia. destruct H10, H3, H3.
+      destruct (length vs) eqn:P0.
+      + apply length_zero_iff_nil in P0. subst.
+        eapply frame_indep_nil in H5 as H5_1.
+        eapply (terminates_step_any_2 _ _ _ _ PP) in H5_1 as H5'.
+        inversion H5'; subst; try inversion_is_value.
+        apply H in H16. 2: lia. destruct H16, H6, H6.
+        assert (⟨ [FApp2 (EFun vl e1) [] []], x2 ⟩ -[1]-> ⟨ [], e1.[list_subst (EFun vl e1 :: [] ++ [x2]) idsubst] ⟩).
+        { repeat econstructor; auto. }
+        eapply frame_indep_nil in H7.
+        epose proof (transitive_eval _ _ _ _ _ H10 _ _ _ H7).
+        assert (⟨ [FApp1 [e]], EFun vl e1 ⟩ -[1]-> ⟨ [FApp2 (EFun vl e1) [] []], e ⟩). { do 2 econstructor; auto. }
+        eapply frame_indep_nil in H2.
+        epose proof (transitive_eval _ _ _ _ _ H2 _ _ _ H16).
+        eapply frame_indep_nil in H5.
+        epose proof (transitive_eval _ _ _ _ _ H5 _ _ _ H10).
+        epose proof (transitive_eval _ _ _ _ _ H17 _ _ _ H18).
+        epose proof (transitive_eval _ _ _ _ _ H19 _ _ _ H7).
+        exists x0, (S (x1 + 1 + (x3 + 1) + x4)). split; auto.
+        econstructor. constructor. auto.
+        inversion H1.
+        apply -> subst_preserves_scope_exp; eauto; subst.
+        simpl. apply cons_scope; auto. rewrite H14. apply cons_scope; auto.
+      + apply eq_sym, last_element_exists in P0. destruct P0, H6. subst.
+        eapply frame_indep_nil in H5 as H5_1.
+        eapply (terminates_step_any_2 _ _ _ _ PP) in H5_1 as H5'.
+
+        epose proof (eval_app_partial_core_emtpy x4 [] x0 x5 _ _ _ _ _ _ _ H5' H3 ltac:(auto)).
+        destruct H6, H6, H6, H7. simpl in H10.
+        eapply frame_indep_core in H10 as H10_1. simpl in H10_1.
+        eapply (terminates_step_any_2 _ _ _ _ H5') in H10_1 as H7'.
+        apply H in H7' as H7''. 2: lia. destruct H7'', H11, H11.
+        eapply frame_indep_nil in H12 as H12_1.
+        eapply (terminates_step_any_2 _ _ _ _ H7') in H12_1 as H11'.
+        inversion H11'; subst; try inversion_is_value.
+        apply H in H21. 2: lia. destruct H21, H13, H13.
+        eapply frame_indep_nil in H12.
+        epose proof (transitive_eval _ _ _ _ _ H10 _ _ _ H12).
+        assert (⟨ [FApp2 (EFun vl e1) [] (x2 :: x7)], x8 ⟩ -[1]->
+              ⟨ [], e1.[list_subst (EFun vl e1 :: (x2 :: x7) ++ [x8]) idsubst] ⟩). { econstructor. constructor; auto. constructor. }
+        epose proof (transitive_eval _ _ _ _ _ H15 _ _ _ H18).
+        epose proof (transitive_eval _ _ _ _ _ H21 _ _ _ H14).
+        eapply frame_indep_nil in H5.
+        epose proof (transitive_eval _ _ _ _ _ H5 _ _ _ H22).
+        assert (⟨ [FApp1 (e :: x4 ++ [x5])], EFun vl e1 ⟩ -[1]->
+            ⟨ [FApp2 (EFun vl e1) (x4 ++ [x5]) []] , e ⟩).
+            { econstructor. constructor. auto. constructor. }
+        simpl app in *.
+        epose proof (transitive_eval _ _ _ _ _ H24 _ _ _ H23).
+        eapply frame_indep_nil in H2.
+        epose proof (transitive_eval _ _ _ _ _ H2 _ _ _ H25).
+
+        exists x0, (S (x1 + (1 + (x3 + (x6 + x9 + 1 + x10))))). split; auto.
+        econstructor. constructor. auto.
+     Unshelve.
+       ** inversion H1. subst. apply -> subst_preserves_scope_exp; eauto.
+          replace (S (Datatypes.length vl) + 0) with (length ((EFun vl e1 :: (x2 :: x7) ++ [x8]))). 2: { simpl. rewrite app_length. simpl in *. lia. }
+          apply scoped_list_idsubst. simpl. do 2 constructor; auto.
+          apply Forall_app; auto.
+        ** inversion P. 2: inversion_is_value.
+           subst. rewrite <- indexed_to_forall in H14.
+           inversion H14. subst. rewrite Forall_app in H16; auto.
+           destruct H16. now inversion H12.
+        ** inversion P. 2: inversion_is_value.
+           rewrite <- indexed_to_forall in H11. now inversion H11.
+        ** inversion P. 2: inversion_is_value.
+           rewrite <- indexed_to_forall in H11. inversion H11.
+           now rewrite Forall_app in H15.
+        ** intros. eapply H. 3: exact H10. lia. auto.
+      + inversion P. 2: inversion_is_value. apply (H7 0); simpl; lia.
+    - now inversion P.
+  * inversion P; subst. 2: inversion_is_value.
+    apply H in H4 as HH; auto. destruct HH as [v0 [k0 [v0CL HH]]].
+    eapply frame_indep_nil in HH as HH0.
+    eapply (terminates_step_any_2 _ _ _ _ H4) in HH0 as HH'.
+    inversion HH'; subst; try inversion_is_value; auto.
+    destruct (length tl) eqn:Len.
+    - apply length_zero_iff_nil in Len. subst.
+      apply H in H9 as H9'; auto. 2: lia.
+      destruct H9' as [hd' [k1 [hd'Vcl H9']]].
+      eapply frame_indep_nil in H9' as H9'0.
+      eapply (terminates_step_any_2 _ _ _ _ H9) in H9'0 as H9''.
+      inversion H9''; subst; try inversion_is_value.
+      inversion P; subst. apply (H10 0 ltac:(simpl;lia)).
+      inversion_is_value.
+    - apply eq_sym, last_element_exists in Len as [tl' [lst ?]]; subst.
+      inversion P; subst; try inversion_is_value.
+      apply indexed_to_forall in H10.
+      inversion H10. subst. apply Forall_app in H12 as [H12_1 H12_2].
+      inversion H12_2; subst.
+      apply H in H9 as H9'; auto. 2: lia.
+      destruct H9' as [hd' [k1 [hd'Vcl H9']]].
+      eapply frame_indep_nil in H9' as H9'0.
+      eapply (terminates_step_any_2 _ _ _ _ H9) in H9'0 as H9''.
+      epose proof (term_bif_eval_empty tl' Fs v0 [] lst hd' _ _ H9'' _ _ _).
+      destruct H1 as [k2 [vals' [Hlt [Hall Der]]]].
+      eapply frame_indep_core in Der as Der0.
+      eapply (terminates_step_any_2 _ _ _ _ H9'') in Der0 as Der'.
+      eapply H in Der' as Der''; auto. 2: lia.
+      destruct Der'' as [lstval [k3 [VCl3 Der'']]].
+      eapply frame_indep_nil in Der'' as Der''0.
+      epose proof (transitive_eval _ _ _ _ _ Der _ _ _ Der''0) as DEND.
+      simpl app in *.
+      eapply frame_indep_nil in H9'.
+      epose proof (transitive_eval _ _ _ _ _ H9' _ _ _ DEND) as COMP.
+      assert (⟨ FBIF1 (hd :: tl' ++ [lst]) :: [], v0 ⟩ -[1]->
+              ⟨ FBIF2 v0 (tl' ++ [lst]) [] :: [], hd ⟩) as ONE. {
+        econstructor. constructor. auto. constructor.
+      }
+      epose proof (transitive_eval _ _ _ _ _ ONE _ _ _ COMP) as COMP'.
+      eapply frame_indep_nil in HH.
+      epose proof (transitive_eval _ _ _ _ _ HH _ _ _ COMP') as COMP''.
+      simpl in COMP''.
+      eapply frame_indep_nil in Der''.
+      eapply (terminates_step_any_2 _ _ _ _ Der') in Der'' as Der'''.
+      inversion Der'''; subst; try inversion_is_value.
+      exists (ELit (i1 + i2)%Z). eexists.
+      split; auto.
+      econstructor. constructor.
+      eapply transitive_eval. exact COMP''.
+      econstructor. constructor. constructor.
+    Unshelve.
+      all: auto.
+      intros. eapply H. 3: exact H14. lia. auto.
+  * apply H in H4 as HH. destruct HH, H1, H1. 2: lia.
+    eapply frame_indep_nil in H2 as H2_1.
+    eapply (terminates_step_any_2 _ _ _ _ H4) in H2_1 as H2'.
+    inversion H2'; subst; try inversion_is_value.
+    apply H in H10 as HH. destruct HH, H3, H3. 2: lia.
+    eapply frame_indep_nil in H5 as H5_1.
+    eapply (terminates_step_any_2 _ _ _ _ H10) in H5_1 as H5'.
+    exists x2, (S (x1 + (S x3))).
+    split. auto.
+    econstructor. constructor. eapply transitive_eval; eauto.
+    eapply frame_indep_nil in H2. exact H2. 
+    econstructor. constructor; auto. auto.
+
+    inversion P. 2: inversion_is_value. 
     apply -> subst_preserves_scope_exp; eauto.
-  * inversion H0. subst. inversion H5. inversion H9. subst. split; auto. constructor; auto.
-    constructor; auto.
-    apply Forall_app. split; auto.
-  * inversion H1. inversion H6. split. auto. subst. inversion H11.
-    apply -> subst_preserves_scope_exp; eauto. subst.
-    rewrite Nat.add_0_r. replace (S (length vl)) with (length (EFun vl e :: vs ++ [v])).
-    apply scoped_list_idsubst. constructor. auto. apply Forall_app. split; auto.
-    simpl. rewrite H0, app_length. simpl. lia.
-  * inversion H0. subst. inversion H4. inversion H3. subst. split; auto.
-    constructor; auto. constructor; auto.
-  * inversion H2. inversion H6. inversion H12.
-    subst. split; auto.
-    constructor; auto. constructor; auto.
-    apply Forall_app. split; auto.
-  * inversion H0. inversion H4. 
-    subst. split; auto. apply -> subst_preserves_scope_exp; eauto.
-  * inversion H1. inversion H5. subst. split; auto.
-    apply -> subst_preserves_scope_exp; eauto.
-    rewrite (match_pattern_length _ v l H0).
-    apply scoped_list_idsubst. eapply match_pattern_scoped; eauto.
-  * inversion H2. inversion H6. subst. split; auto.
-  * inversion H0. inversion H4; subst. split; auto. constructor; auto.
-    constructor. destruct v; inversion H; inversion H1; auto.
-  * inversion H. inversion H3. subst. split; auto. constructor. constructor.
-  * split; auto. inversion H0. 2: inversion H1. apply -> subst_preserves_scope_exp; eauto.
-    subst. apply cons_scope; auto. constructor. auto.
-  * inversion H0. inversion H4. subst. split; auto. repeat constructor; auto.
-  * inversion H1. inversion H5. subst. split; auto. repeat constructor; auto.
-  * inversion H0. 2: inversion H1. subst. split; auto. constructor; auto.
-    now constructor.
-  * inversion H0. 2: inversion H1. subst. split; auto. constructor; auto.
-    constructor. rewrite indexed_to_forall. exact H4.
-  * inversion H0. 2: inversion H1. subst. split; auto. constructor; auto.
-    constructor. rewrite indexed_to_forall. exact H4.
-  * inversion H0. 2: inversion H1. subst. split; auto. constructor; auto. now constructor.
-  * inversion H0. 2: inversion H1. subst. split; auto. constructor; auto.
-    constructor. rewrite Nat.add_0_r in H6. auto. auto.
-  * inversion H0; subst; split; auto. 1-2: constructor; auto; now constructor.
-    now inversion H1.
+    now inversion P.
+  * apply H in H4 as HH. 2: lia. 2: now inversion P.
+    destruct HH as [v2 [k2 [V2CL Eval2]]].
+    eapply frame_indep_nil in Eval2 as Eval2'.
+    eapply (terminates_step_any_2 _ _ _ _ H4) in Eval2'.
+    inversion Eval2'; subst; try inversion_is_value.
+    apply H in H7 as [v1 [k1 [V1CL Eval1]]]. 2: lia. 2: now inversion P.
+    assert (⟨ [FCons1 e1], v2 ⟩ -[1]-> ⟨ [FCons2 v2], e1 ⟩).
+    { econstructor. constructor. auto. constructor. }
+    eapply transitive_eval in H1.
+    2: eapply frame_indep_nil in Eval2 as Eval2''; exact Eval2''.
+    eapply frame_indep_nil in Eval1 as Eval1''.
+    eapply transitive_eval in Eval1''. 2: exact H1.
+    assert (⟨ [FCons2 v2], v1 ⟩ -[1]-> ⟨ [], VCons v1 v2 ⟩).
+    { econstructor. constructor; auto. constructor. }
+    eapply transitive_eval in H2. 2: exact Eval1''.
+    exists (VCons v1 v2), (S ((k2 + 1 + k1) + 1)). split. constructor; auto.
+    econstructor. constructor; auto. exact H2.
 Qed.
 
-Theorem result_VALCLOSED_any (fs : FrameStack) (e v : Exp) :
-  ⟨ fs, e ⟩ -->* v -> VALCLOSED v.
+Corollary term_eval : forall x Fs e (P : EXPCLOSED e), | Fs, e | x ↓ ->
+  exists v k, VALCLOSED v /\ ⟨ Fs, e ⟩ -[k]-> ⟨ Fs, v ⟩ (* /\ k <= x *).
 Proof.
-  intros. destruct H. auto.
+  intros.
+  pose proof (term_eval_empty x Fs e P H).
+  destruct H0, H0, H0.
+  do 2 eexists. split; eauto. eapply frame_indep_nil in H1. exact H1.
 Qed.
 
-Corollary step_any_closedness : forall F e v,
-   ⟨ F, e ⟩ -->* v -> FSCLOSED F -> EXPCLOSED e
-->
-  VALCLOSED v.
+Corollary term_eval_both : forall x Fs e (P : EXPCLOSED e), | Fs, e | x ↓ ->
+  exists v k, VALCLOSED v /\ ⟨ [], e ⟩ -[k]-> ⟨ [], v ⟩ /\ ⟨ Fs, e ⟩ -[k]-> ⟨ Fs, v ⟩.
 Proof.
-  intros. destruct H, H2. induction H2.
-  * destruct e; try inversion H; now inversion H1.
-  * apply step_closedness in H2; auto.
-Qed.
-*)
+  intros. apply term_eval_empty in H. destruct H, H, H.
+  exists x0, x1; split; [| split]; auto.
+  eapply frame_indep_nil in H0; eauto. auto.
+Qed.*)
 
+Lemma params_eval :
+  forall vals ident vl exps e Fs (v : Val),
+  ⟨ FParams ident vl ((map VVal vals) ++ e :: exps) :: Fs, RValSeq [v]⟩ -[length vals]->
+  ⟨ FParams ident (vl ++ vals) exps :: Fs, e⟩.
+Proof.
+
+Admitted.
+
+Lemma params_eval_create :
+  forall vals ident vl Fs (v : Val),
+  ⟨ FParams ident vl (map VVal vals) :: Fs, RValSeq [v]⟩ -[1 + 2 * length vals]->
+  ⟨ Fs, create_result ident (vl ++ v :: vals)⟩.
+Proof.
+  induction vals; simpl; intros.
+  * econstructor. constructor. reflexivity. constructor.
+  (* * destruct (IHvals ident (vl ++ [v]) Fs a) as [k HD]. *)
+  * specialize (IHvals ident (vl ++ [v]) Fs a).
+    econstructor. constructor.
+    econstructor. constructor.
+    rewrite <- app_assoc in IHvals.
+    replace (length vals + S (length vals + 0)) with
+            (1 + 2*length vals) by lia. exact IHvals.
+Qed.
+
+Theorem put_back : forall F e Fs (P : EXPCLOSED e) (P2 : FCLOSED F),
+  | F :: Fs, e | ↓ -> | Fs, plug_f F e | ↓.
+Proof.
+  destruct F; intros; simpl.
+  all: try now (inv H; exists (S x); constructor; auto).
+  * inv H. exists (3 + x). now do 3 constructor.
+  * inv H. destruct ident; simpl.
+    - destruct vl; simpl.
+      + eexists. do 2 constructor. eassumption.
+      + eexists. do 3 constructor.
+        eapply step_term_term; admit.
+  * inv H. destruct lv. (* RBox is not handled by params_eval_create! *)
+    - eexists.
+      do 2 constructor. cbn. eapply cool_params_0. reflexivity.
+      destruct_scopes. inv H6.
+      econstructor. exact H.
+      rewrite eclosed_ignores_sub; auto. exact H0.
+    - exists (6 + ((2 * length lv) + x)). do 2 constructor.
+      simpl. do 2 constructor.
+      eapply step_term_term.
+      apply params_eval_create. 2: lia.
+      replace (S (S (Datatypes.length lv + (Datatypes.length lv + 0) + x)) -
+      (1 + 2 * Datatypes.length lv)) with (S x) by lia.
+      simpl. destruct_scopes. inv H6.
+      econstructor. eassumption. rewrite eclosed_ignores_sub; auto.
+Qed.
+
+Theorem put_back_rev : forall F e Fs (P : EXPCLOSED e), FCLOSED F ->
+  | Fs, plug_f F e | ↓ -> | F :: Fs, e | ↓.
+Proof.
+  destruct F; intros; simpl.
+  all: try now (inv H0; cbn in *; inv H1; [inv H0|eexists;eassumption]).
+  * inv H0. cbn in *. inv H1. inv H0. inv H5. inv H2. eexists. eassumption.
+  * cbn. inv H0. admit.
+  * inv H0. cbn in *. admit.
+Qed.
